[C$] Turn parser state into "shallow" stobj.
Here "shallow" means that the `fty::defprod` has been turned into a stobj, but
its fields are the same, mostly lists, as the `fty::defprod` field, so those
lists are `cons`ed and such. But the parser state itself is updated
destructively.

Since the generated stobj operations do not fix their inputs and do not return
unconditionally typed outputs, we define our own fixtype-like operations that
wrap them. We also introduce a fixtype for the stobj itself. A few
read-over-write theorems (for the fixtype-like readers and writers, not the
stobj-generated ones) were also necessary.

Although the parser code was already written to treat the parser state in a
single-threaded way, this required a number of mostly systematic changes.

We plan to "deepen" the stobj, by turning the list fields into arrays and
indices.

Even with just this shallow stobj, on an example that was taking a while to
parse we get a 2x reduction in time and a 10x reduction in memory usage.

Tests and test macros also had to be adapted, in particular to use
`assert!-stobj`.

books/kestrel/c/syntax/parser.lisp
@@ -498,15 +498,25 @@
 
 ;;;;;;;;;;;;;;;;;;;;;;;;;;;;;;;;;;;;;;;;;;;;;;;;;;;;;;;;;;;;;;;;;;;;;;;;;;;;;;;;
 
-(fty::defprod parstate
+(defsection parstate
   :short "Fixtype of parser states."
   :long
   (xdoc::topstring
    (xdoc::p
     "Our parsing functions take and return parser states.")
    (xdoc::p
+    "The parser state is a stobj, which we turn into a fixtype
+     by adding a fixer along with readers and writers
+     that fix their inputs and unconditionally return typed outputs.
+     The use of a stobj is an optimization for speed:
+     conceptually, the parser state could be defined as a @(tsee fty::defprod),
+     and in fact it was defined like that in previous versions of the parser.
+     The description below of the parser state treats the parser state
+     as if it were defined via @(tsee fty::defprod), not as a stobj;
+     at the end, we explain how the stobj represents that parser state.")
+   (xdoc::p
     "The primary component of a parser state
-     is the input sequence of bytes remaining,
+     is the input sequence @('bytes') of bytes remaining,
      which initially comes from a file (see @(see files)).
      Bytes are read and removed from this component,
      and turned into characters.")
@@ -653,11 +663,6 @@
      This parser state component could potentially evolve into
      a richer set of options for different versions and dialects of C.")
    (xdoc::p
-    "We could look into turning the parser state into a stobj in the future,
-     if efficiency is an issue.
-     The code of the parser already treats the parser state
-     in a single-threaded way.")
-   (xdoc::p
     "For speed, we cache the value returned by
      the function @(tsee parsize) defined later.
      Some profiling revealed that significant time was spent there,
@@ -671,55 +676,365 @@
      The checkpointing and backtracking mechanism described above
      calculates that length in order to record it as a checkpoint.
      When there is a significant number of read token, that can take time,
-     as revealed by some profiling."))
-  ((bytes byte-list)
-   (position position)
-   (chars-read char+position-list)
-   (chars-unread char+position-list)
-   (tokens-read token+span-list)
-   (tokens-read-len natp
-                    :reqfix (len tokens-read))
-   (tokens-unread token+span-list)
-   (checkpoints nat-list)
-   (gcc bool)
-   (size natp
-         :reqfix (+ (len bytes)
-                    (len chars-unread)
-                    (len tokens-unread))))
-  :require (and (equal size
-                       (+ (len bytes)
-                          (len chars-unread)
-                          (len tokens-unread)))
-                (equal tokens-read-len
-                       (len tokens-read)))
-  :pred parstatep
-  :prepwork ((local (in-theory (enable nfix)))))
-
-;;;;;;;;;;;;;;;;;;;;
-
-(defmacro+ irr-parstate ()
-  :short "An irrelevant parser state."
-  :long
-  (xdoc::topstring
+     as revealed by some profiling.")
    (xdoc::p
-    "This is used in functions that take a parser state as input,
-     so a natural choice for an irrelevant parser state to return
-     is the result of fixing the input parser state.")
+    "The stobj for the parser state consists of
+     the components described above,
+     but in a stobj instead of a @(tsee fty::defprod).
+     This is a ``shallow'' stobj, because several of the components
+     are still lists that are updated in a non-destructive way.
+     We plan to ``deepen'' the stobj by using arrays and indices
+     to simulate those lists in a more efficient way.")
    (xdoc::p
-    "This macro assumes that the variable @('parstate') is in scope
-     and has the type of parser states.
-     This is normally a function formal."))
-  '(parstate-fix parstate))
+    "The definition of the stobj itself is straightforward,
+     but we use a @(tsee make-event) so we can use @(tsee position-init)
+     instead of a term for its value that exposes
+     the internal representation of positions.")
+   (xdoc::p
+    "The @(tsee defstobj) generates an enabled recognizer,
+     which we disable after introducing the readers and writers.
+     We define a fixer for that recognizer,
+     using @(tsee mbe) to avoid the stobj restriction
+     of having to return the stobj on all paths.
+     Then we define a fixtype with the same name as the stobj,
+     which causes no issue because fixtypes and stobjs
+     are in different name spaces.
+     In defining the fixtype,
+     we set the equivalence relation to be non-executable,
+     because otherwise we run into stobj restrictions.")
+   (xdoc::p
+    "The @(tsee defstobj) also generates recognizers for the fields,
+     for which we have no use.
+     But we rename them to less ambiguous names,
+     by incorporating @('parstate') into them,
+     to avoid polluting the name space.
+     These recognizers are enabled, but we do not bother disabling them,
+     because we are not going to use them anywhere anyhow.")
+   (xdoc::p
+    "The @(tsee defstobj) also generates readers and writers for the fields,
+     but they neither fix their inputs
+     nor return outputs with unconditional types.
+     So we define our own readers and writers that do both things,
+     which we define in terms of the generated ones.
+     The generated ones are enabled,
+     but we do not both disabling them,
+     because we are not going to use them anywhere anyhow.
+     We also prove some theorems about how readers and writers interact,
+     as needed.")
+   (xdoc::p
+    "We locally enable @(tsee length) in order for
+     the proofs generated by @(tsee defstobj) to go through.
+     This is also useful for proofs about our readers and writers;
+     for those, we also locally enable the fixer.")
+   (xdoc::p
+    "By making the parser state a stobj instead of a @(tsee fty::defprod),
+     we cannot use the @(':require') feature of @(tsee fty::defprod)
+     to enforce that the two redundant components described above
+     are indeed redundant.
+     But we can probably use @(tsee defabsstobj) for that,
+     which may be also overall a better way to
+     ``turn'' a stobj into a @(tsee fty::defprod)-like fixtype."))
+
+  ;; needed for DEFSTOBJ and writer proofs:
+
+  (local (in-theory (enable length)))
+
+  ;; stobj definition:
+
+  (make-event
+   `(defstobj parstate
+      (bytes :type (satisfies byte-listp)
+             :initially nil)
+      (position :type (satisfies positionp)
+                :initially ,(position-init))
+      (chars-read :type (satisfies char+position-listp)
+                  :initially nil)
+      (chars-unread :type (satisfies char+position-listp)
+                    :initially nil)
+      (tokens-read :type (satisfies token+span-listp)
+                   :initially nil)
+      (tokens-read-len :type (integer 0 *)
+                       :initially 0)
+      (tokens-unread :type (satisfies token+span-listp)
+                     :initially nil)
+      (checkpoints :type (satisfies nat-listp)
+                   :initially nil)
+      (gcc :type (satisfies booleanp)
+           :initially nil)
+      (size :type (integer 0 *)
+            :initially 0)
+      :renaming (;; field recognizers:
+                 (bytesp raw-parstate->bytes-p)
+                 (positionp raw-parstate->position-p)
+                 (chars-readp raw-parstate->chars-read-p)
+                 (chars-unreadp raw-parstate->chars-unread-p)
+                 (tokens-readp raw-parstate->tokens-read-p)
+                 (tokens-read-lenp raw-parstate->tokens-read-len-p)
+                 (tokens-unreadp raw-parstate->tokens-unread-p)
+                 (checkpointsp raw-parstate->checkpoints-p)
+                 (gccp raw-parstate->gcc-p)
+                 (sizep raw-parstate->size-p)
+                 ;; field readers:
+                 (bytes raw-parstate->bytes)
+                 (position raw-parstate->position)
+                 (chars-read raw-parstate->chars-read)
+                 (chars-unread raw-parstate->chars-unread)
+                 (tokens-read raw-parstate->tokens-read)
+                 (tokens-read-len raw-parstate->tokens-read-len)
+                 (tokens-unread raw-parstate->tokens-unread)
+                 (checkpoints raw-parstate->checkpoints)
+                 (gcc raw-parstate->gcc)
+                 (size raw-parstate->size)
+                 ;; field writers:
+                 (update-bytes raw-update-parstate->bytes)
+                 (update-position raw-update-parstate->position)
+                 (update-chars-read raw-update-parstate->chars-read)
+                 (update-chars-unread raw-update-parstate->chars-unread)
+                 (update-tokens-read raw-update-parstate->tokens-read)
+                 (update-tokens-read-len raw-update-parstate->tokens-read-len)
+                 (update-tokens-unread raw-update-parstate->tokens-unread)
+                 (update-checkpoints raw-update-parstate->checkpoints)
+                 (update-gcc raw-update-parstate->gcc)
+                 (update-size raw-update-parstate->size))))
+
+  ;; fixer:
+
+  (define parstate-fix (parstate)
+    :returns (parstate parstatep)
+    (mbe :logic (if (parstatep parstate)
+                    parstate
+                  (create-parstate))
+         :exec parstate)
+    ///
+    (defrule parstate-fix-when-parstatep
+      (implies (parstatep parstate)
+               (equal (parstate-fix parstate)
+                      parstate))))
+
+  ;; fixtype:
+
+  (fty::deffixtype parstate
+    :pred parstatep
+    :fix parstate-fix
+    :equiv parstate-equiv
+    :define t
+    :executablep nil)
+
+  ;; needed for readers and writers proofs:
+
+  (local (in-theory (enable parstate-fix)))
+
+  ;; readers:
+
+  (define parstate->bytes (parstate)
+    :returns (bytes byte-listp)
+    (mbe :logic (if (parstatep parstate)
+                    (raw-parstate->bytes parstate)
+                  nil)
+         :exec (raw-parstate->bytes parstate))
+    :hooks (:fix)
+    ///
+    (more-returns
+     (bytes true-listp :rule-classes :type-prescription)))
+
+  (define parstate->position (parstate)
+    :returns (position positionp)
+    (mbe :logic (if (parstatep parstate)
+                    (raw-parstate->position parstate)
+                  (position-init))
+         :exec (raw-parstate->position parstate))
+    :hooks (:fix))
+
+  (define parstate->chars-read (parstate)
+    :returns (chars-read char+position-listp)
+    (mbe :logic (if (parstatep parstate)
+                    (raw-parstate->chars-read parstate)
+                  nil)
+         :exec (raw-parstate->chars-read parstate))
+    :hooks (:fix))
+
+  (define parstate->chars-unread (parstate)
+    :returns (chars-unread char+position-listp)
+    (mbe :logic (if (parstatep parstate)
+                    (raw-parstate->chars-unread parstate)
+                  nil)
+         :exec (raw-parstate->chars-unread parstate))
+    :hooks (:fix))
+
+  (define parstate->tokens-read (parstate)
+    :returns (tokens-read token+span-listp)
+    (mbe :logic (if (parstatep parstate)
+                    (raw-parstate->tokens-read parstate)
+                  nil)
+         :exec (raw-parstate->tokens-read parstate))
+    :hooks (:fix))
+
+  (define parstate->tokens-read-len (parstate)
+    :returns (tokens-read-len natp :rule-classes (:rewrite :type-prescription))
+    (mbe :logic (if (parstatep parstate)
+                    (raw-parstate->tokens-read-len parstate)
+                  0)
+         :exec (raw-parstate->tokens-read-len parstate))
+    :hooks (:fix))
+
+  (define parstate->tokens-unread (parstate)
+    :returns (tokens-unread token+span-listp)
+    (mbe :logic (if (parstatep parstate)
+                    (raw-parstate->tokens-unread parstate)
+                  nil)
+         :exec (raw-parstate->tokens-unread parstate))
+    :hooks (:fix))
+
+  (define parstate->checkpoints (parstate)
+    :returns (checkpoints nat-listp)
+    (mbe :logic (if (parstatep parstate)
+                    (raw-parstate->checkpoints parstate)
+                  nil)
+         :exec (raw-parstate->checkpoints parstate))
+    :hooks (:fix))
+
+  (define parstate->gcc (parstate)
+    :returns (gcc booleanp)
+    (mbe :logic (if (parstatep parstate)
+                    (raw-parstate->gcc parstate)
+                  nil)
+         :exec (raw-parstate->gcc parstate))
+    :hooks (:fix))
+
+  (define parstate->size (parstate)
+    :returns (size natp :rule-classes (:rewrite :type-prescription))
+    (mbe :logic (if (parstatep parstate)
+                    (raw-parstate->size parstate)
+                  0)
+         :exec (raw-parstate->size parstate))
+    :hooks (:fix))
+
+  ;; writers:
+
+  (define update-parstate->bytes ((bytes byte-listp) parstate)
+    :returns (parstate parstatep)
+    (b* ((parstate (parstate-fix parstate)))
+      (raw-update-parstate->bytes (byte-list-fix bytes) parstate))
+    :hooks (:fix))
+
+  (define update-parstate->position ((position positionp) parstate)
+    :returns (parstate parstatep)
+    (b* ((parstate (parstate-fix parstate)))
+      (raw-update-parstate->position (position-fix position) parstate))
+    :hooks (:fix))
+
+  (define update-parstate->chars-read ((chars-read char+position-listp)
+                                       parstate)
+    :returns (parstate parstatep)
+    (b* ((parstate (parstate-fix parstate)))
+      (raw-update-parstate->chars-read (char+position-list-fix chars-read)
+                                       parstate))
+    :hooks (:fix))
+
+  (define update-parstate->chars-unread ((chars-unread char+position-listp)
+                                         parstate)
+    :returns (parstate parstatep)
+    (b* ((parstate (parstate-fix parstate)))
+      (raw-update-parstate->chars-unread (char+position-list-fix chars-unread)
+                                         parstate))
+    :hooks (:fix))
+
+  (define update-parstate->tokens-read ((tokens-read token+span-listp)
+                                        parstate)
+    :returns (parstate parstatep)
+    (b* ((parstate (parstate-fix parstate)))
+      (raw-update-parstate->tokens-read (token+span-list-fix tokens-read)
+                                        parstate))
+    :hooks (:fix))
+
+  (define update-parstate->tokens-read-len ((tokens-read-len natp) parstate)
+    :returns (parstate parstatep)
+    (b* ((parstate (parstate-fix parstate)))
+      (raw-update-parstate->tokens-read-len (lnfix tokens-read-len)
+                                            parstate))
+    :hooks (:fix))
+
+  (define update-parstate->tokens-unread ((tokens-unread token+span-listp)
+                                          parstate)
+    :returns (parstate parstatep)
+    (b* ((parstate (parstate-fix parstate)))
+      (raw-update-parstate->tokens-unread (token+span-list-fix tokens-unread)
+                                          parstate))
+    :hooks (:fix))
+
+  (define update-parstate->checkpoints ((checkpoints nat-listp) parstate)
+    :returns (parstate parstatep)
+    (b* ((parstate (parstate-fix parstate)))
+      (raw-update-parstate->checkpoints (nat-list-fix checkpoints)
+                                        parstate))
+    :hooks (:fix))
+
+  (define update-parstate->gcc ((gcc booleanp) parstate)
+    :returns (parstate parstatep)
+    (b* ((parstate (parstate-fix parstate)))
+      (raw-update-parstate->gcc (bool-fix gcc) parstate))
+    :hooks (:fix))
+
+  (define update-parstate->size ((size natp) parstate)
+    :returns (parstate parstatep)
+    (b* ((parstate (parstate-fix parstate)))
+      (raw-update-parstate->size (lnfix size) parstate))
+    :hooks (:fix))
+
+  ;; readers over writers:
+
+  (defrule parstate->size-of-update-parstate->tokens-read
+    (equal (parstate->size (update-parstate->tokens-read tokens-read parstate))
+           (parstate->size parstate))
+    :enable (parstate->size
+             update-parstate->tokens-read
+             parstatep
+             parstate-fix
+             length))
+
+  (defrule parstate->size-of-update-parstate->tokens-read-len
+    (equal (parstate->size
+            (update-parstate->tokens-read-len tokens-read-len parstate))
+           (parstate->size parstate))
+    :enable (parstate->size
+             update-parstate->tokens-read-len
+             parstatep
+             parstate-fix
+             length))
+
+  (defrule parstate->size-of-update-parstate->checkpoints
+    (equal (parstate->size
+            (update-parstate->checkpoints checkpoints parstate))
+           (parstate->size parstate))
+    :enable (parstate->size
+             update-parstate->checkpoints
+             parstatep
+             parstate-fix
+             length))
+
+  (defrule parstate->size-of-update-parstate->size
+    (equal (parstate->size (update-parstate->size size parstate))
+           (lnfix size))
+    :enable (parstate->size
+             update-parstate->size
+             parstatep
+             parstate-fix
+             length))
+
+  ;; keep recognizer disabled:
+
+  (in-theory (disable parstatep)))
 
 ;;;;;;;;;;;;;;;;;;;;;;;;;;;;;;;;;;;;;;;;
 
-(define init-parstate ((data byte-listp) (gcc booleanp))
+(define init-parstate ((data byte-listp) (gcc booleanp) parstate)
   :returns (parstate parstatep)
-  :short "Initial parser state."
+  :short "Initialize the parser state."
   :long
   (xdoc::topstring
    (xdoc::p
-    "Given (the data of) a file to parse,
+    "This is the state when we start parsing a file.
+     Given (the data of) a file to parse,
      and a flag saying whether GCC extensions should be accepted or not,
      the initial parsing state consists of
      the data to parse,
@@ -727,42 +1042,69 @@
      no read characters or tokens,
      the initial file position,
      and no checkpoints."))
-  (make-parstate :bytes data
-                 :position (position-init)
-                 :chars-read nil
-                 :chars-unread nil
-                 :tokens-read nil
-                 :tokens-read-len 0
-                 :tokens-unread nil
-                 :checkpoints nil
-                 :gcc gcc
-                 :size (len data))
-  :guard-hints (("Goal" :in-theory (enable fix))))
+  (b* ((parstate (update-parstate->bytes data parstate))
+       (parstate (update-parstate->position (position-init) parstate))
+       (parstate (update-parstate->chars-read nil parstate))
+       (parstate (update-parstate->chars-unread nil parstate))
+       (parstate (update-parstate->tokens-read nil parstate))
+       (parstate (update-parstate->tokens-read-len 0 parstate))
+       (parstate (update-parstate->tokens-unread nil parstate))
+       (parstate (update-parstate->checkpoints nil parstate))
+       (parstate (update-parstate->gcc gcc parstate))
+       (parstate (update-parstate->size (len data) parstate)))
+    parstate)
+  :hooks (:fix))
 
 ;;;;;;;;;;;;;;;;;;;;;;;;;;;;;;;;;;;;;;;;
 
 (define parsize ((parstate parstatep))
-  :returns (size natp)
+  :returns (size natp :rule-classes (:rewrite :type-prescription))
   :short "Size of the parsing state."
   :long
   (xdoc::topstring
    (xdoc::p
-    "This is used as the measure for termination of the parsing functions.
-     The size is measured as the sum of
-     the lists of bytes, characters, and tokens that can be read.")
-   (xdoc::p
-    "As explained in @(tsee parstate), this is cached for efficiency.
-     We use an @(tsee mbe) to just return the value in execution."))
-  (mbe :logic (+ (len (parstate->bytes parstate))
-                 (len (parstate->chars-unread parstate))
-                 (len (parstate->tokens-unread parstate)))
-       :exec (parstate->size parstate))
+    "This is a synonym of @(tsee parstate->size) at this point.
+     It was slightly more elaborate when
+     @(tsee parstate) was defined via @(tsee fty::defprod)."))
+  (parstate->size parstate)
+  :hooks (:fix)
 
   ///
 
-  (defrule parsize-of-parstate-fix
-    (equal (parsize (parstate-fix parstate))
-           (parsize parstate))))
+  (defrule parsize-of-initparstate
+    (equal (parsize (init-parstate nil gcc parstate))
+           0)
+    :enable init-parstate))
+
+;;;;;;;;;;;;;;;;;;;;;;;;;;;;;;;;;;;;;;;;
+
+; fixtype version of PARSTATE stobj (useful for debugging and testing)
+(fty::defprod parstate$
+  ((bytes byte-list)
+   (position position)
+   (chars-read char+position-list)
+   (chars-unread char+position-list)
+   (tokens-read token+span-list)
+   (tokens-read-len nat)
+   (tokens-unread token+span-list)
+   (checkpoints nat-list)
+   (gcc bool)
+   (size nat))
+  :prepwork ((local (in-theory (enable nfix)))))
+
+; convert PARSTATE stobj to fixtype value (useful for debugging and testing)
+(define to-parstate$ (parstate)
+  (make-parstate$
+   :bytes (parstate->bytes parstate)
+   :position (parstate->position parstate)
+   :chars-read (parstate->chars-read parstate)
+   :chars-unread (parstate->chars-unread parstate)
+   :tokens-read (parstate->tokens-read parstate)
+   :tokens-read-len (parstate->tokens-read-len parstate)
+   :tokens-unread (parstate->tokens-unread parstate)
+   :checkpoints (parstate->checkpoints parstate)
+   :gcc (parstate->gcc parstate)
+   :size (parstate->size parstate)))
 
 ;;;;;;;;;;;;;;;;;;;;;;;;;;;;;;;;;;;;;;;;;;;;;;;;;;;;;;;;;;;;;;;;;;;;;;;;;;;;;;;;
 
@@ -892,7 +1234,10 @@
 ;;;;;;;;;;;;;;;;;;;;;;;;;;;;;;;;;;;;;;;;;;;;;;;;;;;;;;;;;;;;;;;;;;;;;;;;;;;;;;;;
 
 (define read-char ((parstate parstatep))
-  :returns (mv erp (char? nat-optionp) (pos positionp) (new-parstate parstatep))
+  :returns (mv erp
+               (char? nat-optionp)
+               (pos positionp)
+               (new-parstate parstatep :hyp (parstatep parstate)))
   :short "Read a character."
   :long
   (xdoc::topstring
@@ -1014,19 +1359,26 @@
      just increment the column number by 1 and leave the line number unchanged.
      This may not be appropriate for certain Unicode characters,
      but for now we treat them in this simplified way."))
-  (b* (((reterr) nil (irr-position) (irr-parstate))
-       ((parstate parstate) parstate)
-       ((when (consp parstate.chars-unread))
-        (b* ((char+pos (car parstate.chars-unread)))
+  (b* (((reterr) nil (irr-position) parstate)
+       (parstate.bytes (parstate->bytes parstate))
+       (parstate.position (parstate->position parstate))
+       (parstate.chars-read (parstate->chars-read parstate))
+       (parstate.chars-unread (parstate->chars-unread parstate))
+       (parstate.size (parstate->size parstate))
+       ((when (and (consp parstate.chars-unread)
+                   (> parstate.size 0)))
+        (b* ((char+pos (car parstate.chars-unread))
+             (parstate (update-parstate->chars-unread
+                        (cdr parstate.chars-unread) parstate))
+             (parstate (update-parstate->chars-read
+                        (cons char+pos parstate.chars-read) parstate))
+             (parstate (update-parstate->size (1- parstate.size) parstate)))
           (retok (char+position->char char+pos)
                  (char+position->position char+pos)
-                 (change-parstate
-                  parstate
-                  :chars-unread (cdr parstate.chars-unread)
-                  :chars-read (cons char+pos parstate.chars-read)
-                  :size (1- parstate.size)))))
-       ((unless (consp parstate.bytes))
-        (retok nil parstate.position (parstate-fix parstate)))
+                 parstate)))
+       ((unless (and (consp parstate.bytes)
+                     (> parstate.size 0)))
+        (retok nil parstate.position parstate))
        (byte (car parstate.bytes))
        (bytes (cdr parstate.bytes))
        ;; ASCII except line feed and carriage return:
@@ -1034,50 +1386,53 @@
                   (= byte 11)
                   (= byte 12)
                   (and (<= 32 byte) (<= byte 126))))
-        (retok byte
-               parstate.position
-               (change-parstate
-                parstate
-                :bytes bytes
-                :position (position-inc-column 1 parstate.position)
-                :chars-read (cons (make-char+position
-                                   :char byte
-                                   :position parstate.position)
-                                  parstate.chars-read)
-                :size (1- parstate.size))))
+        (b* ((parstate (update-parstate->bytes bytes parstate))
+             (parstate (update-parstate->position
+                        (position-inc-column 1 parstate.position) parstate))
+             (parstate (update-parstate->chars-read
+                        (cons (make-char+position
+                               :char byte
+                               :position parstate.position)
+                              parstate.chars-read)
+                        parstate))
+             (parstate (update-parstate->size (1- parstate.size) parstate)))
+          (retok byte parstate.position parstate)))
        ;; line feed:
        ((when (= byte 10))
-        (retok 10
-               parstate.position
-               (change-parstate
-                parstate
-                :bytes bytes
-                :position (position-inc-line 1 parstate.position)
-                :chars-read (cons (make-char+position
-                                   :char 10
-                                   :position parstate.position)
-                                  parstate.chars-read)
-                :size (1- parstate.size))))
+        (b* ((parstate (update-parstate->bytes bytes parstate))
+             (parstate (update-parstate->position
+                        (position-inc-line 1 parstate.position) parstate))
+             (parstate (update-parstate->chars-read
+                        (cons (make-char+position
+                               :char 10
+                               :position parstate.position)
+                              parstate.chars-read)
+                        parstate))
+             (parstate (update-parstate->size (1- parstate.size) parstate)))
+          (retok 10 parstate.position parstate)))
        ;; carriage return:
        ((when (= byte 13))
         (b* (((mv bytes count) (if (and (consp bytes)
+                                        (> parstate.size 1)
                                         (= (car bytes) 10))
                                    (mv (cdr bytes) 2)
-                                (mv bytes 1))))
-          (retok 10
-                 parstate.position
-                 (change-parstate
-                  parstate
-                  :bytes bytes
-                  :position (position-inc-line 1 parstate.position)
-                  :chars-read (cons (make-char+position
-                                     :char 10
-                                     :position parstate.position)
-                                    parstate.chars-read)
-                  :size (- parstate.size count)))))
+                                 (mv bytes 1)))
+             (parstate (update-parstate->bytes bytes parstate))
+             (parstate (update-parstate->position
+                        (position-inc-line 1 parstate.position) parstate))
+             (parstate (update-parstate->chars-read
+                        (cons (make-char+position
+                               :char 10
+                               :position parstate.position)
+                              parstate.chars-read)
+                        parstate))
+             (parstate (update-parstate->size
+                        (- parstate.size count) parstate)))
+          (retok 10 parstate.position parstate)))
        ;; 2-byte UTF-8:
        ((when (= (logand byte #b11100000) #b11000000)) ; 110xxxyy
-        (b* (((unless (consp bytes))
+        (b* (((unless (and (consp bytes)
+                           (> parstate.size 1)))
               (reterr-msg :where (position-to-msg parstate.position)
                           :expected (msg "another byte after ~
                                           the first byte ~x0 ~
@@ -1106,21 +1461,22 @@
                                           UTF-8-encoded in the two bytes ~
                                           (~x0 ~x1)"
                                          byte byte2)
-                          :found (msg "the value ~x0" code))))
-          (retok code
-                 parstate.position
-                 (change-parstate
-                  parstate
-                  :bytes bytes
-                  :position (position-inc-column 1 parstate.position)
-                  :chars-read (cons (make-char+position
-                                     :char code
-                                     :position parstate.position)
-                                    parstate.chars-read)
-                  :size (- parstate.size 2)))))
+                          :found (msg "the value ~x0" code)))
+             (parstate (update-parstate->bytes bytes parstate))
+             (parstate (update-parstate->position
+                        (position-inc-column 1 parstate.position) parstate))
+             (parstate (update-parstate->chars-read
+                        (cons (make-char+position
+                               :char code
+                               :position parstate.position)
+                              parstate.chars-read)
+                        parstate))
+             (parstate (update-parstate->size (- parstate.size 2) parstate)))
+          (retok code parstate.position parstate)))
        ;; 3-byte UTF-8:
        ((when (= (logand byte #b11110000) #b11100000)) ; 1110xxxx
-        (b* (((unless (consp bytes))
+        (b* (((unless (and (consp bytes)
+                           (> parstate.size 1)))
               (reterr-msg :where (position-to-msg parstate.position)
                           :expected (msg "another byte after ~
                                           the first byte ~x0 ~
@@ -1141,7 +1497,8 @@
                                           of a three-byte UTF-8 encoding"
                                          byte)
                           :found (msg "the byte ~x0" byte2)))
-             ((unless (consp bytes))
+             ((unless (and (consp bytes)
+                           (> parstate.size 2)))
               (reterr-msg :where (position-to-msg parstate.position)
                           :expected (msg "another byte after ~
                                           the first byte ~x0 ~
@@ -1187,21 +1544,22 @@
                                      in the range 9-13 or 32-126 ~
                                      or 128-8233 or 8239-8293 or ~
                                      or 8298-55295 or 57344-1114111"
-                          :found (char-to-msg code))))
-          (retok code
-                 parstate.position
-                 (change-parstate
-                  parstate
-                  :bytes bytes
-                  :position (position-inc-column 1 parstate.position)
-                  :chars-read (cons (make-char+position
-                                     :char code
-                                     :position parstate.position)
-                                    parstate.chars-read)
-                  :size (- parstate.size 3)))))
+                          :found (char-to-msg code)))
+             (parstate (update-parstate->bytes bytes parstate))
+             (parstate (update-parstate->position
+                        (position-inc-column 1 parstate.position) parstate))
+             (parstate (update-parstate->chars-read
+                        (cons (make-char+position
+                               :char code
+                               :position parstate.position)
+                              parstate.chars-read)
+                        parstate))
+             (parstate (update-parstate->size (- parstate.size 3) parstate)))
+          (retok code parstate.position parstate)))
        ;; 4-byte UTF-8:
        ((when (= (logand #b11111000 byte) #b11110000)) ; 11110xyy
-        (b* (((unless (consp bytes))
+        (b* (((unless (and (consp bytes)
+                           (> parstate.size 1)))
               (reterr-msg :where (position-to-msg parstate.position)
                           :expected (msg "another byte after ~
                                           the first byte ~x0 ~
@@ -1222,7 +1580,8 @@
                                           of a four-byte UTF-8 encoding"
                                          byte)
                           :found (msg "the byte ~x0" byte2)))
-             ((unless (consp bytes))
+             ((unless (and (consp bytes)
+                           (> parstate.size 2)))
               (reterr-msg :where (position-to-msg parstate.position)
                           :expected (msg "another byte after ~
                                           the first byte ~x0 ~
@@ -1249,7 +1608,8 @@
                                           of a four-byte UTF-8 encoding"
                                          byte byte2)
                           :found (msg "the byte ~x0" byte3)))
-             ((unless (consp bytes))
+             ((unless (and (consp bytes)
+                           (> parstate.size 3)))
               (reterr-msg :where (position-to-msg parstate.position)
                           :expected (msg "another byte after ~
                                           the first byte ~x0 ~
@@ -1293,30 +1653,33 @@
                                           UTF-8-encoded in the four bytes ~
                                           (~x0 ~x1 ~x2 ~x3)"
                                          byte byte2 byte3 byte4)
-                          :found (msg "the value ~x0" code))))
-          (retok code
-                 parstate.position
-                 (change-parstate
-                  parstate
-                  :bytes bytes
-                  :position (position-inc-column 1 parstate.position)
-                  :chars-read (cons (make-char+position
-                                     :char code
-                                     :position parstate.position)
-                                    parstate.chars-read)
-                  :size (- parstate.size 4))))))
+                          :found (msg "the value ~x0" code)))
+             (parstate (update-parstate->bytes bytes parstate))
+             (parstate (update-parstate->position
+                        (position-inc-column 1 parstate.position) parstate))
+             (parstate (update-parstate->chars-read
+                        (cons (make-char+position
+                               :char code
+                               :position parstate.position)
+                              parstate.chars-read)
+                        parstate))
+             (parstate (update-parstate->size (- parstate.size 4) parstate)))
+          (retok code parstate.position parstate))))
     (reterr-msg :where (position-to-msg parstate.position)
                 :expected "a byte in the range 9-13 or 32-126 or 192-223"
                 :found (msg "the byte ~x0" byte)))
   :guard-hints (("Goal" :in-theory (e/d (len fix natp)
                                         ((:e tau-system))))) ; for speed
   :prepwork ((local (in-theory (enable acl2-numberp-when-bytep
+                                       acl2-numberp-when-natp
                                        rationalp-when-bytep
+                                       rationalp-when-natp
                                        integerp-when-natp
                                        natp-when-bytep
                                        natp-of-plus
                                        natp-of-logand
-                                       natp-of-ash))))
+                                       natp-of-ash)))
+             (local (include-book "arithmetic/top" :dir :system)))
 
   ///
 
@@ -1324,7 +1687,7 @@
     (<= (parsize new-parstate)
         (parsize parstate))
     :rule-classes :linear
-    :hints (("Goal" :in-theory (enable parsize len))))
+    :hints (("Goal" :in-theory (enable parsize len nfix))))
 
   (defret parsize-of-read-char-cond
     (implies (and (not erp)
@@ -1332,12 +1695,12 @@
              (<= (parsize new-parstate)
                  (1- (parsize parstate))))
     :rule-classes :linear
-    :hints (("Goal" :in-theory (enable parsize len fix)))))
+    :hints (("Goal" :in-theory (enable parsize len fix nfix)))))
 
 ;;;;;;;;;;;;;;;;;;;;;;;;;;;;;;;;;;;;;;;;
 
 (define unread-char ((parstate parstatep))
-  :returns (new-parstate parstatep)
+  :returns (new-parstate parstatep :hyp (parstatep parstate))
   :short "Unread a character."
   :long
   (xdoc::topstring
@@ -1351,32 +1714,38 @@
      logically we return a parser state
      where we push an irrelevant character and position,
      so that the theorem about @(tsee parsize) holds unconditionally."))
-  (b* (((parstate parstate) parstate)
+  (b* ((parstate.chars-read (parstate->chars-read parstate))
+       (parstate.chars-unread (parstate->chars-unread parstate))
+       (parstate.size (parstate->size parstate))
        ((unless (consp parstate.chars-read))
         (raise "Internal error: no character to unread.")
-        (change-parstate parstate
-                         :chars-unread (cons (make-char+position
-                                              :char 0
-                                              :position (irr-position))
-                                             parstate.chars-unread)
-                         :size (1+ parstate.size)))
-       (char+pos (car parstate.chars-read)))
-    (change-parstate parstate
-                     :chars-unread (cons char+pos parstate.chars-unread)
-                     :chars-read (cdr parstate.chars-read)
-                     :size (1+ parstate.size)))
+        (b* ((parstate (update-parstate->chars-unread
+                        (cons (make-char+position
+                               :char 0
+                               :position (irr-position))
+                              parstate.chars-unread)
+                        parstate))
+             (parstate (update-parstate->size (1+ parstate.size) parstate)))
+          parstate))
+       (char+pos (car parstate.chars-read))
+       (parstate (update-parstate->chars-unread
+                  (cons char+pos parstate.chars-unread) parstate))
+       (parstate (update-parstate->chars-read
+                  (cdr parstate.chars-read) parstate))
+       (parstate (update-parstate->size (1+ parstate.size) parstate)))
+    parstate)
 
   ///
 
   (defret parsize-of-unread-char
     (equal (parsize new-parstate)
            (1+ (parsize parstate)))
-    :hints (("Goal" :in-theory (enable parsize len)))))
+    :hints (("Goal" :in-theory (enable parsize len nfix)))))
 
 ;;;;;;;;;;;;;;;;;;;;;;;;;;;;;;;;;;;;;;;;
 
 (define unread-chars ((n natp) (parstate parstatep))
-  :returns (new-parstate parstatep)
+  :returns (new-parstate parstatep :hyp (parstatep parstate))
   :short "Unread a specified number of characters."
   :long
   (xdoc::topstring
@@ -1408,7 +1777,10 @@
              (and (<= (char-code #\a) first-char)
                   (<= first-char (char-code #\z)))
              (= first-char (char-code #\_)))
-  :returns (mv erp (lexeme lexemep) (span spanp) (new-parstate parstatep))
+  :returns (mv erp
+               (lexeme lexemep)
+               (span spanp)
+               (new-parstate parstatep :hyp (parstatep parstate)))
   :short "Lex an identifier or keyword."
   :long
   (xdoc::topstring
@@ -1447,7 +1819,7 @@
      (more precisely, lists of that).
      If the ASCII string is a keyword, we return a keyword token.
      Otherwise, we return an identifier token."))
-  (b* (((reterr) (irr-lexeme) (irr-span) (irr-parstate))
+  (b* (((reterr) (irr-lexeme) (irr-span) parstate)
        ((erp rest-chars last-pos parstate)
         (lex-identifier/keyword-loop first-pos parstate))
        (span (make-span :start first-pos :end last-pos))
@@ -1522,9 +1894,9 @@
                                                      integer-range-p
                                                      integerp-when-natp))))
                   (last-pos positionp)
-                  (new-parstate parstatep))
+                  (new-parstate parstatep :hyp (parstatep parstate)))
      :parents nil
-     (b* (((reterr) nil (irr-position) (irr-parstate))
+     (b* (((reterr) nil (irr-position) parstate)
           ((erp char pos parstate) (read-char parstate))
           ((when (not char))
            (retok nil (position-fix pos-so-far) parstate))
@@ -1571,7 +1943,7 @@
                                                    integer-range-p
                                                    integerp-when-natp))))
                (pos positionp)
-               (new-parstate parstatep))
+               (new-parstate parstatep :hyp (parstatep parstate)))
   :short "Lex a hexadecimal digit."
   :long
   (xdoc::topstring
@@ -1581,7 +1953,7 @@
      If the next character is present and is a hexadecimal digit,
      we return the corresponding ACL2 character,
      along with its position in the file."))
-  (b* (((reterr) #\0 (irr-position) (irr-parstate))
+  (b* (((reterr) #\0 (irr-position) parstate)
        ((erp char pos parstate) (read-char parstate))
        ((when (not char))
         (reterr-msg :where (position-to-msg pos)
@@ -1619,7 +1991,7 @@
   :returns (mv erp
                (quad hex-quad-p)
                (last-pos positionp)
-               (new-parstate parstatep))
+               (new-parstate parstatep :hyp (parstatep parstate)))
   :short "Lex a quadruple of hexadecimal digits."
   :long
   (xdoc::topstring
@@ -1627,7 +1999,7 @@
     "This is called when we expect four hexadecimal digits,
      so we call @(tsee lex-hexadecimal-digit) four times.
      We return the position of the last one."))
-  (b* (((reterr) (irr-hex-quad) (irr-position) (irr-parstate))
+  (b* (((reterr) (irr-hex-quad) (irr-position) parstate)
        ((erp hexdig1 & parstate) (lex-hexadecimal-digit parstate))
        ((erp hexdig2 & parstate) (lex-hexadecimal-digit parstate))
        ((erp hexdig3 & parstate) (lex-hexadecimal-digit parstate))
@@ -1667,7 +2039,7 @@
                                              integerp-when-natp))))
                (last-pos positionp)
                (next-pos positionp)
-               (new-parstate parstatep))
+               (new-parstate parstatep :hyp (parstatep parstate)))
   :short "Lex zero or more (decimal) digits, as many as available."
   :long
   (xdoc::topstring
@@ -1692,7 +2064,7 @@
      or the input @('pos-so-far') if there is no digit:
      this input is the position read so far,
      just before the zero or more digits to be read."))
-  (b* (((reterr) nil (irr-position) (irr-position) (irr-parstate))
+  (b* (((reterr) nil (irr-position) (irr-position) parstate)
        ((erp char pos parstate) (read-char parstate))
        ((when (not char))
         (retok nil (position-fix pos-so-far) pos parstate))
@@ -1737,7 +2109,7 @@
                                              integerp-when-natp))))
                (last-pos positionp)
                (next-pos positionp)
-               (new-parstate parstatep))
+               (new-parstate parstatep :hyp (parstatep parstate)))
   :short "Lex zero or more hexadecimal digits, as many as available."
   :long
   (xdoc::topstring
@@ -1762,7 +2134,7 @@
      or the input @('pos-so-far') if there is no hexadecimal character:
      this input is the position read so far,
      just before the zero or more hexadecimal digits to be read."))
-  (b* (((reterr) nil (irr-position) (irr-position) (irr-parstate))
+  (b* (((reterr) nil (irr-position) (irr-position) parstate)
        ((erp char pos parstate) (read-char parstate))
        ((when (not char))
         (retok nil (position-fix pos-so-far) pos parstate))
@@ -1803,7 +2175,7 @@
   :returns (mv erp
                (escape escapep)
                (last-pos positionp)
-               (new-parstate parstatep))
+               (new-parstate parstatep :hyp (parstatep parstate)))
   :short "Lex an escape sequence."
   :long
   (xdoc::topstring
@@ -1834,7 +2206,7 @@
     "In all other cases, it is an error:
      although this starts like an escape sequence,
      it is not one."))
-  (b* (((reterr) (irr-escape) (irr-position) (irr-parstate))
+  (b* (((reterr) (irr-escape) (irr-position) parstate)
        ((erp char pos parstate) (read-char parstate)))
     (cond
      ((not char)
@@ -1951,7 +2323,7 @@
   :returns (mv erp
                (cchars c-char-listp)
                (closing-squote-pos positionp)
-               (new-parstate parstatep))
+               (new-parstate parstatep :hyp (parstatep parstate)))
   :short "Lex zero or more characters and escape sequences
           in a character constant."
   :long
@@ -1978,7 +2350,7 @@
      we take the character as is,
      we read zero or more additional characters and escape sequences,
      and we combine them with the character."))
-  (b* (((reterr) nil (irr-position) (irr-parstate))
+  (b* (((reterr) nil (irr-position) parstate)
        ((erp char pos parstate) (read-char parstate))
        ((unless char)
         (reterr-msg :where (position-to-msg pos)
@@ -2030,7 +2402,7 @@
   :returns (mv erp
                (schars s-char-listp)
                (closing-dquote-pos positionp)
-               (new-parstate parstatep))
+               (new-parstate parstatep :hyp (parstatep parstate)))
   :short "Lex zero or more characters and escape sequences
           in a string literal."
   :long
@@ -2057,7 +2429,7 @@
      we take the character as is,
      we read zero or more additional characters and escape sequences,
      and we combine them with the character."))
-  (b* (((reterr) nil (irr-position) (irr-parstate))
+  (b* (((reterr) nil (irr-position) parstate)
        ((erp char pos parstate) (read-char parstate))
        ((unless char)
         (reterr-msg :where (position-to-msg pos)
@@ -2108,7 +2480,10 @@
 (define lex-character-constant ((cprefix? cprefix-optionp)
                                 (first-pos positionp)
                                 (parstate parstatep))
-  :returns (mv erp (lexeme lexemep) (span spanp) (new-parstate parstatep))
+  :returns (mv erp
+               (lexeme lexemep)
+               (span spanp)
+               (new-parstate parstatep :hyp (parstatep parstate)))
   :short "Lex a character constant."
   :long
   (xdoc::topstring
@@ -2123,7 +2498,7 @@
      we read up to the closing single quote (see @(tsee lex-*-c-char)),
      whose position we use as the ending one of the span we return.
      The starting position of the span is passed to this function as input."))
-  (b* (((reterr) (irr-lexeme) (irr-span) (irr-parstate))
+  (b* (((reterr) (irr-lexeme) (irr-span) parstate)
        ((erp cchars closing-squote-pos parstate) (lex-*-c-char parstate))
        (span (make-span :start first-pos :end closing-squote-pos))
        ((unless cchars)
@@ -2152,7 +2527,10 @@
 (define lex-stringlit ((eprefix? eprefix-optionp)
                        (first-pos positionp)
                        (parstate parstatep))
-  :returns (mv erp (lexeme lexemep) (span spanp) (new-parstate parstatep))
+  :returns (mv erp
+               (lexeme lexemep)
+               (span spanp)
+               (new-parstate parstatep :hyp (parstatep parstate)))
   :short "Lex a string literal."
   :long
   (xdoc::topstring
@@ -2166,7 +2544,7 @@
      we read up to the closing double quote (see @(tsee lex-*-s-char)),
      whose position we use as the ending one of the span we return.
      The starting position of the span is passed to this function as input."))
-  (b* (((reterr) (irr-lexeme) (irr-span) (irr-parstate))
+  (b* (((reterr) (irr-lexeme) (irr-span) parstate)
        ((erp schars closing-dquote-pos parstate) (lex-*-s-char parstate))
        (span (make-span :start first-pos :end closing-dquote-pos)))
     (retok (lexeme-token (token-string (stringlit eprefix? schars)))
@@ -2192,7 +2570,7 @@
   :returns (mv erp
                (isuffix? isuffix-optionp)
                (last/next-pos positionp)
-               (new-parstate parstatep))
+               (new-parstate parstatep :hyp (parstatep parstate)))
   :short "Lex an integer suffix, if present."
   :long
   (xdoc::topstring
@@ -2228,7 +2606,7 @@
      We could shorten it by merging the treatment of
      lowercase @('l') and uppercase @('L'),
      single or double."))
-  (b* (((reterr) nil (irr-position) (irr-parstate))
+  (b* (((reterr) nil (irr-position) parstate)
        ((erp char pos parstate) (read-char parstate)))
     (cond
      ((not char) ; EOF
@@ -2422,7 +2800,7 @@
   :returns (mv erp
                (fsuffix? fsuffix-optionp)
                (last/next-pos positionp)
-               (new-parstate parstatep))
+               (new-parstate parstatep :hyp (parstatep parstate)))
   :short "Lex a floating suffix, if present."
   :long
   (xdoc::topstring
@@ -2434,7 +2812,7 @@
      Otherwise, there are four possibilities for suffixes.
      If the next character is not part of any suffix,
      we unread the character and return no suffix."))
-  (b* (((reterr) nil (irr-position) (irr-parstate))
+  (b* (((reterr) nil (irr-position) parstate)
        ((erp char pos parstate) (read-char parstate)))
     (cond
      ((not char)
@@ -2472,7 +2850,7 @@
   :returns (mv erp
                (sign? sign-optionp)
                (last/next-pos positionp)
-               (new-parstate parstatep))
+               (new-parstate parstatep :hyp (parstatep parstate)))
   :short "Lex a sign, if present."
   :long
   (xdoc::topstring
@@ -2484,7 +2862,7 @@
      Otherwise, we read the next character,
      and return a sign if appropriate,
      otherwise no sign and we put back the character."))
-  (b* (((reterr) nil (irr-position) (irr-parstate))
+  (b* (((reterr) nil (irr-position) parstate)
        ((erp char pos parstate) (read-char parstate)))
     (cond
      ((not char)
@@ -2518,7 +2896,7 @@
   :returns (mv erp
                (expo? dec-expo-optionp)
                (last/next-pos positionp)
-               (new-parstate parstatep))
+               (new-parstate parstatep :hyp (parstatep parstate)))
   :short "Lex a decimal exponent, if present."
   :long
   (xdoc::topstring
@@ -2536,7 +2914,7 @@
      we put back the sign character (if it was present),
      and we put back the @('e') or @('E').
      If there are digits, we return an appropriate exponent."))
-  (b* (((reterr) nil (irr-position) (irr-parstate))
+  (b* (((reterr) nil (irr-position) parstate)
        ((erp char pos parstate) (read-char parstate)))
     (cond
      ((not char)
@@ -2585,7 +2963,7 @@
   :returns (mv erp
                (expo dec-expop)
                (last-pos positionp)
-               (new-parstate parstatep))
+               (new-parstate parstatep :hyp (parstatep parstate)))
   :short "Lex a decimal exponent."
   :long
   (xdoc::topstring
@@ -2595,7 +2973,7 @@
      Then we read an optional sign.
      Then we read zero or more decimal digits,
      of which there must be at least one."))
-  (b* (((reterr) (irr-dec-expo) (irr-position) (irr-parstate))
+  (b* (((reterr) (irr-dec-expo) (irr-position) parstate)
        ((erp char pos parstate) (read-char parstate)))
     (cond
      ((not char)
@@ -2646,7 +3024,7 @@
   :returns (mv erp
                (expo bin-expop)
                (last-pos positionp)
-               (new-parstate parstatep))
+               (new-parstate parstatep :hyp (parstatep parstate)))
   :short "Lex a binary exponent."
   :long
   (xdoc::topstring
@@ -2656,7 +3034,7 @@
      Then we read an optional sign.
      Then we read zero or more decimal digits,
      of which there must be at least one."))
-  (b* (((reterr) (irr-bin-expo) (irr-position) (irr-parstate))
+  (b* (((reterr) (irr-bin-expo) (irr-position) parstate)
        ((erp char pos parstate) (read-char parstate)))
     (cond
      ((not char)
@@ -2705,7 +3083,7 @@
 
 (define check-full-ppnumber ((ends-in-e booleanp)
                              (parstate parstatep))
-  :returns (mv erp (new-parstate parstatep))
+  :returns (mv erp (new-parstate parstatep :hyp (parstatep parstate)))
   :short "Check that the numerical constant just read
           is a full preprocessing number."
   :long
@@ -2794,7 +3172,7 @@
      in particular, @('0xf') is a valid hexadecimal integer constant.
      But @('0xe+1') is not a hexadecimal (or integer) constant,
      and so it cannot be converted to one."))
-  (b* (((reterr) (irr-parstate))
+  (b* (((reterr) parstate)
        ((erp char pos parstate) (read-char parstate))
        ((when (not char)) (retok parstate))
        ((when (or (and (<= (char-code #\A) char)
@@ -2835,7 +3213,7 @@
   :returns (mv erp
                (const constp)
                (last-pos positionp)
-               (new-parstate parstatep))
+               (new-parstate parstatep :hyp (parstatep parstate)))
   :short "Lex a hexadecimal integer or floating constant."
   :long
   (xdoc::topstring
@@ -2872,7 +3250,7 @@
     "Just before returning the constant,
      we use @(tsee check-full-ppnumber),
      for the reasons explained there."))
-  (b* (((reterr) (irr-const) (irr-position) (irr-parstate))
+  (b* (((reterr) (irr-const) (irr-position) parstate)
        ;; 0 x/X
        ((erp hexdigs hexdigs-last-pos & parstate)
         (lex-*-hexadecimal-digit prefix-last-pos parstate)))
@@ -3039,7 +3417,7 @@
   :returns (mv erp
                (const constp)
                (last-pos positionp)
-               (new-parstate parstatep))
+               (new-parstate parstatep :hyp (parstatep parstate)))
   :short "Lex a decimal integer or floating constant."
   :long
   (xdoc::topstring
@@ -3080,7 +3458,7 @@
      We put back the character and read an integer suffix if present.
      If @(tsee check-full-ppnumber) passes,
      we return the appropriate integer constant."))
-  (b* (((reterr) (irr-const) (irr-position) (irr-parstate))
+  (b* (((reterr) (irr-const) (irr-position) parstate)
        ;; 1-9
        ((erp decdigs decdigs-last-pos & parstate)
         (lex-*-digit first-pos parstate))
@@ -3200,7 +3578,10 @@
 (define lex-dec-fconst ((first-digit-after-dot dec-digit-char-p)
                         (first-pos-after-dot positionp)
                         (parstate parstatep))
-  :returns (mv erp (const constp) (last-pos positionp) (new-parstate parstatep))
+  :returns (mv erp
+               (const constp)
+               (last-pos positionp)
+               (new-parstate parstatep :hyp (parstatep parstate)))
   :short "Lex a decimal floating constant."
   :long
   (xdoc::topstring
@@ -3213,7 +3594,7 @@
      Then a floating suffix, if present.
      Finally, if @(tsee check-full-ppnumber) passes,
      we return an appropriate floating constant."))
-  (b* (((reterr) (irr-const) (irr-position) (irr-parstate))
+  (b* (((reterr) (irr-const) (irr-position) parstate)
        ;; . decdig
        ((erp decdigs decdigs-last-pos & parstate)
         (lex-*-digit first-pos-after-dot parstate))
@@ -3257,7 +3638,10 @@
 ;;;;;;;;;;;;;;;;;;;;;;;;;;;;;;;;;;;;;;;;;;;;;;;;;;;;;;;;;;;;;;;;;;;;;;;;;;;;;;;;
 
 (define lex-non-octal-digit ((parstate parstatep))
-  :returns (mv erp (char natp) (pos positionp) (new-parstate parstatep))
+  :returns (mv erp
+               (char natp)
+               (pos positionp)
+               (new-parstate parstatep :hyp (parstatep parstate)))
   :short "Lex a non-octal digit."
   :long
   (xdoc::topstring
@@ -3271,7 +3655,7 @@
      So we expect that a non-octal digit will be found,
      and it is thus an internal error if it is not found
      (which should never happen)."))
-  (b* (((reterr) 0 (irr-position) (irr-parstate))
+  (b* (((reterr) 0 (irr-position) parstate)
        ((erp char pos parstate) (read-char parstate))
        ((unless char)
         (raise "Internal error: no non-octal digit found.")
@@ -3302,7 +3686,10 @@
 ;;;;;;;;;;;;;;;;;;;;;;;;;;;;;;;;;;;;;;;;;;;;;;;;;;;;;;;;;;;;;;;;;;;;;;;;;;;;;;;;
 
 (define lex-oct-iconst-/-dec-fconst ((zero-pos positionp) (parstate parstatep))
-  :returns (mv erp (const constp) (last-pos positionp) (new-parstate parstatep))
+  :returns (mv erp
+               (const constp)
+               (last-pos positionp)
+               (new-parstate parstatep :hyp (parstatep parstate)))
   :long
   (xdoc::topstring
    (xdoc::p
@@ -3362,7 +3749,7 @@
      because in the latter case the digits would have to be followed by
      a dot or an exponent;
      so it is an error in that case."))
-  (b* (((reterr) (irr-const) (irr-position) (irr-parstate))
+  (b* (((reterr) (irr-const) (irr-position) parstate)
        ;; 0
        ((erp digits digits-last-pos & parstate)
         (lex-*-digit zero-pos parstate))
@@ -3502,7 +3889,10 @@
 (define lex-iconst/fconst ((first-digit dec-digit-char-p)
                            (first-pos positionp)
                            (parstate parstatep))
-  :returns (mv erp (const constp) (last-pos positionp) (new-parstate parstatep))
+  :returns (mv erp
+               (const constp)
+               (last-pos positionp)
+               (new-parstate parstatep :hyp (parstatep parstate)))
   :short "Lex an integer or floating constant."
   :long
   (xdoc::topstring
@@ -3523,7 +3913,7 @@
     "If instead the first digit is @('1') to @('9'),
      we must have a decimal integer or floating constant,
      for which we use a separate function."))
-  (b* (((reterr) (irr-const) (irr-position) (irr-parstate)))
+  (b* (((reterr) (irr-const) (irr-position) parstate))
     (cond
      ((eql first-digit #\0) ; 0
       (b* (((erp char pos parstate) (read-char parstate)))
@@ -3561,7 +3951,10 @@
 ;;;;;;;;;;;;;;;;;;;;;;;;;;;;;;;;;;;;;;;;;;;;;;;;;;;;;;;;;;;;;;;;;;;;;;;;;;;;;;;;
 
 (define lex-block-comment ((first-pos positionp) (parstate parstatep))
-  :returns (mv erp (lexeme lexemep) (span spanp) (new-parstate parstatep))
+  :returns (mv erp
+               (lexeme lexemep)
+               (span spanp)
+               (new-parstate parstatep :hyp (parstatep parstate)))
   :short "Lex a block comment."
   :long
   (xdoc::topstring
@@ -3583,7 +3976,7 @@
      passed to this function,
      and the last position (of the @('/') in the closing @('*/')),
      returned by the loop function."))
-  (b* (((reterr) (irr-lexeme) (irr-span) (irr-parstate))
+  (b* (((reterr) (irr-lexeme) (irr-span) parstate)
        ((erp last-pos parstate) (lex-rest-of-block-comment first-pos parstate)))
     (retok (lexeme-comment)
            (make-span :start first-pos :end last-pos)
@@ -3595,8 +3988,10 @@
 
      (define lex-rest-of-block-comment ((first-pos positionp)
                                         (parstate parstatep))
-       :returns (mv erp (last-pos positionp) (new-parstate parstatep))
-       (b* (((reterr) (irr-position) (irr-parstate))
+       :returns (mv erp
+                    (last-pos positionp)
+                    (new-parstate parstatep :hyp (parstatep parstate)))
+       (b* (((reterr) (irr-position) parstate)
             ((erp char pos parstate) (read-char parstate)))
          (cond
           ((not char) ; EOF
@@ -3614,8 +4009,10 @@
 
      (define lex-rest-of-block-comment-after-star ((first-pos positionp)
                                                    (parstate parstatep))
-       :returns (mv erp (last-pos positionp) (new-parstate parstatep))
-       (b* (((reterr) (irr-position) (irr-parstate))
+       :returns (mv erp
+                    (last-pos positionp)
+                    (new-parstate parstatep :hyp (parstatep parstate)))
+       (b* (((reterr) (irr-position) parstate)
             ((erp char pos parstate) (read-char parstate)))
          (cond
           ((not char) ; EOF
@@ -3681,7 +4078,10 @@
 ;;;;;;;;;;;;;;;;;;;;;;;;;;;;;;;;;;;;;;;;;;;;;;;;;;;;;;;;;;;;;;;;;;;;;;;;;;;;;;;;
 
 (define lex-line-comment ((first-pos positionp) (parstate parstatep))
-  :returns (mv erp (lexeme lexemep) (span spanp) (new-parstate parstatep))
+  :returns (mv erp
+               (lexeme lexemep)
+               (span spanp)
+               (new-parstate parstatep :hyp (parstatep parstate)))
   :short "Lex a line comment."
   :long
   (xdoc::topstring
@@ -3700,7 +4100,7 @@
      which is passed to this function,
      and the position of the closing new-line,
      which is returned by the loop function."))
-  (b* (((reterr) (irr-lexeme) (irr-span) (irr-parstate))
+  (b* (((reterr) (irr-lexeme) (irr-span) parstate)
        ((erp last-pos parstate) (lex-line-comment-loop first-pos parstate)))
     (retok (lexeme-comment)
            (make-span :start first-pos :end last-pos)
@@ -3709,9 +4109,11 @@
   :prepwork
 
   ((define lex-line-comment-loop ((first-pos positionp) (parstate parstatep))
-     :returns (mv erp (last-pos positionp) (new-parstate parstatep))
+     :returns (mv erp
+                  (last-pos positionp)
+                  (new-parstate parstatep :hyp (parstatep parstate)))
      :parents nil
-     (b* (((reterr) (irr-position) (irr-parstate))
+     (b* (((reterr) (irr-position) parstate)
           ((erp char pos parstate) (read-char parstate)))
        (cond
         ((not char) ; EOF
@@ -3763,7 +4165,7 @@
   :returns (mv erp
                (lexeme? lexeme-optionp)
                (span spanp)
-               (new-parstate parstatep))
+               (new-parstate parstatep :hyp (parstatep parstate)))
   :short "Lex a lexeme."
   :long
   (xdoc::topstring
@@ -3887,7 +4289,7 @@
       Some punctuators are not prefixes of others,
       and so they can be immediately decided.")))
 
-  (b* (((reterr) nil (irr-span) (irr-parstate))
+  (b* (((reterr) nil (irr-span) parstate)
        ((erp char first-pos parstate) (read-char parstate))
        ((unless char)
         (retok nil
@@ -4421,7 +4823,7 @@
   :returns (mv erp
                (token? token-optionp)
                (span spanp)
-               (new-parstate parstatep))
+               (new-parstate parstatep :hyp (parstatep parstate)))
   :short "Read a token."
   :long
   (xdoc::topstring
@@ -4446,19 +4848,25 @@
      That is, we discard white space and comments.
      (Future extensions of this parser may instead
      return certain white space and comments under some conditions.)"))
-  (b* (((reterr) nil (irr-span) (irr-parstate))
-       ((parstate parstate) parstate)
-       ((when (consp parstate.tokens-unread))
-        (b* ((token+span (car parstate.tokens-unread)))
+  (b* (((reterr) nil (irr-span) parstate)
+       (parstate.tokens-read (parstate->tokens-read parstate))
+       (parstate.tokens-read-len (parstate->tokens-read-len parstate))
+       (parstate.tokens-unread (parstate->tokens-unread parstate))
+       (parstate.size (parstate->size parstate))
+       ((when (and (consp parstate.tokens-unread)
+                   (> parstate.size 0)))
+        (b* ((token+span (car parstate.tokens-unread))
+             (parstate (update-parstate->tokens-unread
+                        (cdr parstate.tokens-unread) parstate))
+             (parstate (update-parstate->tokens-read
+                        (cons token+span parstate.tokens-read) parstate))
+             (parstate (update-parstate->tokens-read-len
+                        (1+ parstate.tokens-read-len) parstate))
+             (parstate (update-parstate->chars-read nil parstate))
+             (parstate (update-parstate->size (1- parstate.size) parstate)))
           (retok (token+span->token token+span)
                  (token+span->span token+span)
-                 (change-parstate
-                  parstate
-                  :tokens-unread (cdr parstate.tokens-unread)
-                  :tokens-read (cons token+span parstate.tokens-read)
-                  :tokens-read-len (1+ parstate.tokens-read-len)
-                  :chars-read nil
-                  :size (1- parstate.size))))))
+                 parstate))))
     (read-token-loop parstate))
   :guard-hints (("Goal" :in-theory (enable natp fix len)))
 
@@ -4468,22 +4876,23 @@
      :returns (mv erp
                   (token? token-optionp)
                   (span spanp)
-                  (new-parstate parstatep))
+                  (new-parstate parstatep :hyp (parstatep parstate)))
      :parents nil
-     (b* (((reterr) nil (irr-span) (irr-parstate))
+     (b* (((reterr) nil (irr-span) parstate)
           ((erp lexeme? span parstate) (lex-lexeme parstate))
           ((when (not lexeme?))
            (retok nil span parstate))
           ((when (lexeme-case lexeme? :token))
            (b* ((token (lexeme-token->unwrap lexeme?))
-                (parstate (change-parstate
-                         parstate
-                         :tokens-read (cons (make-token+span
-                                             :token token
-                                             :span span)
-                                            (parstate->tokens-read parstate))
-                         :tokens-read-len (1+ (parstate->tokens-read-len
-                                               parstate)))))
+                (parstate (update-parstate->tokens-read
+                           (cons (make-token+span
+                                  :token token
+                                  :span span)
+                                 (parstate->tokens-read parstate))
+                           parstate))
+                (parstate (update-parstate->tokens-read-len
+                           (1+ (parstate->tokens-read-len parstate))
+                           parstate)))
              (retok token span parstate))))
        (read-token-loop parstate))
      :measure (parsize parstate)
@@ -4518,7 +4927,7 @@
         (parsize parstate))
     :rule-classes :linear
     :hints (("Goal"
-             :in-theory (e/d (parsize len fix)
+             :in-theory (e/d (parsize len fix nfix)
                              (parsize-of-read-token-loop-uncond))
              :use parsize-of-read-token-loop-uncond)))
 
@@ -4529,14 +4938,14 @@
                  (1- (parsize parstate))))
     :rule-classes :linear
     :hints (("Goal"
-             :in-theory (e/d (parsize len fix)
+             :in-theory (e/d (parsize len fix nfix)
                              (parsize-of-read-token-loop-cond))
              :use parsize-of-read-token-loop-cond))))
 
 ;;;;;;;;;;;;;;;;;;;;;;;;;;;;;;;;;;;;;;;;
 
 (define unread-token ((parstate parstatep))
-  :returns (new-parstate parstatep)
+  :returns (new-parstate parstatep :hyp (parstatep parstate))
   :short "Unread a token."
   :long
   (xdoc::topstring
@@ -4550,21 +4959,30 @@
      logically we return a parser state
      where we push an irrelevant character and position,
      so that the theorem about @(tsee parsize) holds unconditionally."))
-  (b* (((parstate parstate) parstate)
-       ((unless (consp parstate.tokens-read))
+  (b* ((parstate.tokens-read (parstate->tokens-read parstate))
+       (parstate.tokens-read-len (parstate->tokens-read-len parstate))
+       (parstate.tokens-unread (parstate->tokens-unread parstate))
+       (parstate.size (parstate->size parstate))
+       ((unless (and (consp parstate.tokens-read)
+                     (> parstate.tokens-read-len 0)))
         (raise "Internal error: no token to unread.")
-        (change-parstate parstate
-                         :tokens-unread (cons (make-token+span
-                                               :token (irr-token)
-                                               :span (irr-span))
-                                              parstate.tokens-unread)
-                         :size (1+ parstate.size)))
-       (token+span (car parstate.tokens-read)))
-    (change-parstate parstate
-                     :tokens-unread (cons token+span parstate.tokens-unread)
-                     :tokens-read (cdr parstate.tokens-read)
-                     :tokens-read-len (1- parstate.tokens-read-len)
-                     :size (1+ parstate.size)))
+        (b* ((parstate (update-parstate->tokens-unread
+                        (cons (make-token+span
+                               :token (irr-token)
+                               :span (irr-span))
+                              parstate.tokens-unread)
+                        parstate))
+             (parstate (update-parstate->size (1+ parstate.size) parstate)))
+          parstate))
+       (token+span (car parstate.tokens-read))
+       (parstate (update-parstate->tokens-unread
+                  (cons token+span parstate.tokens-unread) parstate))
+       (parstate (update-parstate->tokens-read
+                  (cdr parstate.tokens-read) parstate))
+       (parstate (update-parstate->tokens-read-len
+                  (1- parstate.tokens-read-len) parstate))
+       (parstate (update-parstate->size (1+ parstate.size) parstate)))
+    parstate)
   :guard-hints (("Goal" :in-theory (enable natp len fix)))
 
   ///
@@ -4572,12 +4990,12 @@
   (defret parsize-of-unread-token
     (equal (parsize new-parstate)
            (1+ (parsize parstate)))
-    :hints (("Goal" :in-theory (enable parsize len)))))
+    :hints (("Goal" :in-theory (enable parsize len nfix)))))
 
 ;;;;;;;;;;;;;;;;;;;;;;;;;;;;;;;;;;;;;;;;
 
 (define unread-tokens ((n natp) (parstate parstatep))
-  :returns (new-parstate parstatep)
+  :returns (new-parstate parstatep :hyp (parstatep parstate))
   :short "Unread a specified number of tokens."
   :long
   (xdoc::topstring
@@ -4602,7 +5020,9 @@
 ;;;;;;;;;;;;;;;;;;;;;;;;;;;;;;;;;;;;;;;;
 
 (define read-punctuator ((punct stringp) (parstate parstatep))
-  :returns (mv erp (span spanp) (new-parstate parstatep))
+  :returns (mv erp
+               (span spanp)
+               (new-parstate parstatep :hyp (parstatep parstate)))
   :short "Read a specific punctuator token."
   :long
   (xdoc::topstring
@@ -4611,7 +5031,7 @@
      We pass the string for the punctuator,
      and we read the next token,
      ensuring it exists and it is that punctuator."))
-  (b* (((reterr) (irr-span) (irr-parstate))
+  (b* (((reterr) (irr-span) parstate)
        ((erp token span parstate) (read-token parstate))
        ((unless (token-punctuatorp token punct)) ; implies non-nil
         (reterr-msg :where (position-to-msg (span->start span))
@@ -4635,7 +5055,9 @@
 ;;;;;;;;;;;;;;;;;;;;;;;;;;;;;;;;;;;;;;;;
 
 (define read-keyword ((keywd stringp) (parstate parstatep))
-  :returns (mv erp (span spanp) (new-parstate parstatep))
+  :returns (mv erp
+               (span spanp)
+               (new-parstate parstatep :hyp (parstatep parstate)))
   :short "Read a specific keyword token."
   :long
   (xdoc::topstring
@@ -4644,7 +5066,7 @@
      We pass the string for the keyword,
      and we read the next token,
      ensuring it exists and it is that keyword."))
-  (b* (((reterr) (irr-span) (irr-parstate))
+  (b* (((reterr) (irr-span) parstate)
        ((erp token span parstate) (read-token parstate))
        ((unless (token-keywordp token keywd)) ; implies non-nil
         (reterr-msg :where (position-to-msg (span->start span))
@@ -4668,7 +5090,10 @@
 ;;;;;;;;;;;;;;;;;;;;;;;;;;;;;;;;;;;;;;;;
 
 (define read-stringlit ((parstate parstatep))
-  :returns (mv erp (stringlit stringlitp) (span spanp) (new-parstate parstatep))
+  :returns (mv erp
+               (stringlit stringlitp)
+               (span spanp)
+               (new-parstate parstatep :hyp (parstatep parstate)))
   :short "Read a string literal token."
   :long
   (xdoc::topstring
@@ -4676,7 +5101,7 @@
     "This is called when we expect a string literal token.
      We read the next token, ensuring it exists and is a string literal.
      We return the string literal if successful."))
-  (b* (((reterr) (irr-stringlit) (irr-span) (irr-parstate))
+  (b* (((reterr) (irr-stringlit) (irr-span) parstate)
        ((erp token span parstate) (read-token parstate))
        ((unless (and token
                      (token-case token :string)))
@@ -4702,7 +5127,10 @@
 ;;;;;;;;;;;;;;;;;;;;;;;;;;;;;;;;;;;;;;;;
 
 (define read-identifier ((parstate parstatep))
-  :returns (mv erp (ident identp) (span spanp) (new-parstate parstatep))
+  :returns (mv erp
+               (ident identp)
+               (span spanp)
+               (new-parstate parstatep :hyp (parstatep parstate)))
   :short "Read an identifier token."
   :long
   (xdoc::topstring
@@ -4710,7 +5138,7 @@
     "This is called when we expect an identifier token.
      We read the next token, ensuring it exists and is an identifier.
      We return the identifier if successful."))
-  (b* (((reterr) (irr-ident) (irr-span) (irr-parstate))
+  (b* (((reterr) (irr-ident) (irr-span) parstate)
        ((erp token span parstate) (read-token parstate))
        ((unless (and token
                      (token-case token :ident)))
@@ -4736,7 +5164,7 @@
 ;;;;;;;;;;;;;;;;;;;;;;;;;;;;;;;;;;;;;;;;;;;;;;;;;;;;;;;;;;;;;;;;;;;;;;;;;;;;;;;;
 
 (define record-checkpoint ((parstate parstatep))
-  :returns (new-parstate parstatep)
+  :returns (new-parstate parstatep :hyp (parstatep parstate))
   :short "Record a checkpoint for possible backtracking."
   :long
   (xdoc::topstring
@@ -4747,8 +5175,8 @@
   (b* ((tokens-read-len (parstate->tokens-read-len parstate))
        (checkpoints (parstate->checkpoints parstate))
        (new-checkpoints (cons tokens-read-len checkpoints))
-       (new-parstate (change-parstate parstate :checkpoints new-checkpoints)))
-    new-parstate)
+       (parstate (update-parstate->checkpoints new-checkpoints parstate)))
+    parstate)
 
   ///
 
@@ -4761,7 +5189,7 @@
 ;;;;;;;;;;;;;;;;;;;;;;;;;;;;;;;;;;;;;;;;
 
 (define clear-checkpoint ((parstate parstatep))
-  :returns (new-parstate parstatep)
+  :returns (new-parstate parstatep :hyp (parstatep parstate))
   :short "Clear the latest checkpoint."
   :long
   (xdoc::topstring
@@ -4775,12 +5203,12 @@
      when the list of checkpoints is empty.
      If this happens, there is a bug in the parser."))
   (b* ((checkpoints (parstate->checkpoints parstate))
-       ((unless checkpoints)
+       ((unless (consp checkpoints))
         (raise "Internal error: no checkpoint to clear.")
         (parstate-fix parstate))
        (new-checkpoints (cdr checkpoints))
-       (new-parstate (change-parstate parstate :checkpoints new-checkpoints)))
-    new-parstate)
+       (parstate (update-parstate->checkpoints new-checkpoints parstate)))
+    parstate)
 
   ///
 
@@ -4793,7 +5221,7 @@
 ;;;;;;;;;;;;;;;;;;;;;;;;;;;;;;;;;;;;;;;;
 
 (define backtrack-checkpoint ((parstate parstatep))
-  :returns (new-parstate parstatep)
+  :returns (new-parstate parstatep :hyp (parstatep parstate))
   :short "Backtrack to the latest checkpoint."
   :long
   (xdoc::topstring
@@ -4822,14 +5250,14 @@
                number-tokens-read)
         (parstate-fix parstate))
        (parstate (unread-tokens number-tokens-to-unread parstate))
-       (new-parstate (change-parstate parstate :checkpoints new-chechpoints)))
-    new-parstate)
+       (parstate (update-parstate->checkpoints new-chechpoints parstate)))
+    parstate)
   :prepwork
   ((defrulel verify-guards-lemma
      (implies (and (natp x)
                    (natp y)
-                   (>= y x))
-              (natp (+ (- x) y)))
+                   (< 0 (+ x (- y))))
+              (natp (+ x (- y))))
      :enable natp)))
 
 ;;;;;;;;;;;;;;;;;;;;;;;;;;;;;;;;;;;;;;;;;;;;;;;;;;;;;;;;;;;;;;;;;;;;;;;;;;;;;;;;
@@ -5731,7 +6159,7 @@
   :returns (mv erp
                (strings stringlit-listp)
                (span spanp)
-               (new-parstate parstatep))
+               (new-parstate parstatep :hyp (parstatep parstate)))
   :short "Parse a list of zero or more string literals."
   :long
   (xdoc::topstring
@@ -5744,7 +6172,7 @@
      we join spans only if the remaining ones are one or more;
      if there are zero, the span of the first string literal
      is also the span of the whole sequence."))
-  (b* (((reterr) nil (irr-span) (irr-parstate))
+  (b* (((reterr) nil (irr-span) parstate)
        ((erp token span parstate) (read-token parstate))
        ((unless (and token (token-case token :string)))
         (b* ((parstate (if token (unread-token parstate) parstate)))
@@ -5774,8 +6202,7 @@
   :returns (mv erp
                (tyquals type-qual-listp)
                (span spanp)
-               (new-parstate parstatep))
-  :parents (parser parse-exprs/decls)
+               (new-parstate parstatep :hyp (parstatep parstate)))
   :short "Parse a list of one or more type qualifiers."
   :long
   (xdoc::topstring
@@ -5784,7 +6211,7 @@
      Then we check the next token to see if there is be another one,
      in which case we put it back and recursively parse a type qualifier list,
      otherwise we put back it back and return."))
-  (b* (((reterr) nil (irr-span) (irr-parstate))
+  (b* (((reterr) nil (irr-span) parstate)
        ((erp token span parstate) (read-token parstate)))
     (cond
      ((token-type-qualifier-p token) ; tyqual
@@ -5836,8 +6263,7 @@
   :returns (mv erp
                (tyqualss type-qual-list-listp)
                (span spanp)
-               (new-parstate parstatep))
-  :parents (parser parse-exprs/decls)
+               (new-parstate parstatep :hyp (parstatep parstate)))
   :short "Parse a pointer."
   :long
   (xdoc::topstring
@@ -5858,7 +6284,7 @@
      If instead the initial star is followed by another star,
      we also call this function recursively.
      We stop when there is not a star."))
-  (b* (((reterr) nil (irr-span) (irr-parstate))
+  (b* (((reterr) nil (irr-span) parstate)
        ((erp span parstate) (read-punctuator "*" parstate)) ; *
        ((erp token & parstate) (read-token parstate)))
     (cond
@@ -5910,7 +6336,9 @@
 ;;;;;;;;;;;;;;;;;;;;;;;;;;;;;;;;;;;;;;;;;;;;;;;;;;;;;;;;;;;;;;;;;;;;;;;;;;;;;;;;
 
 (define parse-*-increment/decrement ((parstate parstatep))
-  :returns (mv erp (ops inc/dec-op-listp) (new-parstate parstatep))
+  :returns (mv erp
+               (ops inc/dec-op-listp)
+               (new-parstate parstatep :hyp (parstatep parstate)))
   :short "Parse zero or more increment and decrement operators."
   :long
   (xdoc::topstring
@@ -5918,7 +6346,7 @@
     "This is used to handle possibly ambiguous cast expressions.
      We never need the spans of these operators,
      so this function returns no span."))
-  (b* (((reterr) nil (irr-parstate))
+  (b* (((reterr) nil parstate)
        ((erp token & parstate) (read-token parstate))
        ((when (token-punctuatorp token "++"))
         (b* (((erp ops parstate) (parse-*-increment/decrement parstate)))
@@ -6011,7 +6439,10 @@
   ;;;;;;;;;;;;;;;;;;;;;;;;;;;;;;;;;;;;;;;;
 
   (define parse-expression ((parstate parstatep))
-    :returns (mv erp (expr exprp) (span spanp) (new-parstate parstatep))
+    :returns (mv erp
+                 (expr exprp)
+                 (span spanp)
+                 (new-parstate parstatep :hyp (parstatep parstate)))
     :parents (parser parse-exprs/decls)
     :short "Parse an expression."
     :long
@@ -6034,7 +6465,7 @@
        to @(tsee parse-expression-rest),
        where the final expression is constructed:
        see the documentation of that function for details."))
-    (b* (((reterr) (irr-expr) (irr-span) (irr-parstate))
+    (b* (((reterr) (irr-expr) (irr-span) parstate)
          (psize (parsize parstate))
          ((erp expr span parstate) (parse-assignment-expression parstate))
          ((unless (mbt (<= (parsize parstate) (1- psize))))
@@ -6047,7 +6478,10 @@
   (define parse-expression-rest ((prev-expr exprp)
                                  (prev-span spanp)
                                  (parstate parstatep))
-    :returns (mv erp (expr exprp) (span spanp) (new-parstate parstatep))
+    :returns (mv erp
+                 (expr exprp)
+                 (span spanp)
+                 (new-parstate parstatep :hyp (parstatep parstate)))
     :parents (parser parse-exprs/decls)
     :short "Parse the rest of an expression."
     :long
@@ -6074,7 +6508,7 @@
        this is the new current expression,
        which we pass to the recursive call of this function.
        Spans are joined similarly."))
-    (b* (((reterr) (irr-expr) (irr-span) (irr-parstate))
+    (b* (((reterr) (irr-expr) (irr-span) parstate)
          ;; prev-expr
          ((erp token & parstate) (read-token parstate))
          ((when (not (token-punctuatorp token ","))) ; prev-expr not,
@@ -6095,7 +6529,10 @@
   ;;;;;;;;;;;;;;;;;;;;;;;;;;;;;;;;;;;;;;;;
 
   (define parse-assignment-expression ((parstate parstatep))
-    :returns (mv erp (expr exprp) (span spanp) (new-parstate parstatep))
+    :returns (mv erp
+                 (expr exprp)
+                 (span spanp)
+                 (new-parstate parstatep :hyp (parstatep parstate)))
     :parents (parser parse-exprs/decls)
     :short "Parse an assignment expression."
     :long
@@ -6117,7 +6554,7 @@
        and instead it is a unary expression,
        which includes unary expressions propers
        but also other kinds of expressions."))
-    (b* (((reterr) (irr-expr) (irr-span) (irr-parstate))
+    (b* (((reterr) (irr-expr) (irr-span) parstate)
          (psize (parsize parstate))
          ((erp expr span parstate)
           (parse-conditional-expression parstate)) ; expr
@@ -6143,7 +6580,10 @@
   ;;;;;;;;;;;;;;;;;;;;;;;;;;;;;;;;;;;;;;;;
 
   (define parse-conditional-expression ((parstate parstatep))
-    :returns (mv erp (expr exprp) (span spanp) (new-parstate parstatep))
+    :returns (mv erp
+                 (expr exprp)
+                 (span spanp)
+                 (new-parstate parstatep :hyp (parstatep parstate)))
     :parents (parser parse-exprs/decls)
     :short "Parse a conditional expression."
     :long
@@ -6157,7 +6597,7 @@
        and then we check whether there is a @('?'):
        if there is, it must be a conditional expression proper;
        if there is not, it must be a logical disjunction expression."))
-    (b* (((reterr) (irr-expr) (irr-span) (irr-parstate))
+    (b* (((reterr) (irr-expr) (irr-span) parstate)
          (psize (parsize parstate))
          ((erp expr span parstate)
           (parse-logical-or-expression parstate)) ; expr
@@ -6183,7 +6623,10 @@
   ;;;;;;;;;;;;;;;;;;;;;;;;;;;;;;;;;;;;;;;;
 
   (define parse-logical-or-expression ((parstate parstatep))
-    :returns (mv erp (expr exprp) (span spanp) (new-parstate parstatep))
+    :returns (mv erp
+                 (expr exprp)
+                 (span spanp)
+                 (new-parstate parstatep :hyp (parstatep parstate)))
     :parents (parser parse-exprs/decls)
     :short "Parse a logical disjunction expression."
     :long
@@ -6192,7 +6635,7 @@
       "We handle the left recursion in the grammar rule
        in the same way as for expressions:
        see @(tsee parse-expression)."))
-    (b* (((reterr) (irr-expr) (irr-span) (irr-parstate))
+    (b* (((reterr) (irr-expr) (irr-span) parstate)
          (psize (parsize parstate))
          ((erp expr span parstate) (parse-logical-and-expression parstate))
          ((unless (mbt (<= (parsize parstate) (1- psize))))
@@ -6205,7 +6648,10 @@
   (define parse-logical-or-expression-rest ((prev-expr exprp)
                                             (prev-span spanp)
                                             (parstate parstatep))
-    :returns (mv erp (expr exprp) (span spanp) (new-parstate parstatep))
+    :returns (mv erp
+                 (expr exprp)
+                 (span spanp)
+                 (new-parstate parstatep :hyp (parstatep parstate)))
     :parents (parser parse-exprs/decls)
     :short "Parse the rest of a logical disjunction expression."
     :long
@@ -6213,7 +6659,7 @@
      (xdoc::p
       "This completes the job started by @(tsee parse-logical-or-expression);
        it is analogous to @(tsee parse-expression-rest)."))
-    (b* (((reterr) (irr-expr) (irr-span) (irr-parstate))
+    (b* (((reterr) (irr-expr) (irr-span) parstate)
          ;; prev-expr
          ((erp token & parstate) (read-token parstate))
          ((when (not (token-punctuatorp token "||"))) ; prev-expr not||
@@ -6236,7 +6682,10 @@
   ;;;;;;;;;;;;;;;;;;;;;;;;;;;;;;;;;;;;;;;;
 
   (define parse-logical-and-expression ((parstate parstatep))
-    :returns (mv erp (expr exprp) (span spanp) (new-parstate parstatep))
+    :returns (mv erp
+                 (expr exprp)
+                 (span spanp)
+                 (new-parstate parstatep :hyp (parstatep parstate)))
     :parents (parser parse-exprs/decls)
     :short "Parse a logical conjunction expression."
     :long
@@ -6245,7 +6694,7 @@
       "We handle the left recursion in the grammar rule
        in the same way as for expressions:
        see @(tsee parse-expression)."))
-    (b* (((reterr) (irr-expr) (irr-span) (irr-parstate))
+    (b* (((reterr) (irr-expr) (irr-span) parstate)
          (psize (parsize parstate))
          ((erp expr span parstate) (parse-inclusive-or-expression parstate))
          ((unless (mbt (<= (parsize parstate) (1- psize))))
@@ -6258,7 +6707,10 @@
   (define parse-logical-and-expression-rest ((prev-expr exprp)
                                              (prev-span spanp)
                                              (parstate parstatep))
-    :returns (mv erp (expr exprp) (span spanp) (new-parstate parstatep))
+    :returns (mv erp
+                 (expr exprp)
+                 (span spanp)
+                 (new-parstate parstatep :hyp (parstatep parstate)))
     :parents (parser parse-exprs/decls)
     :short "Parse the rest of a logical conjunction expression."
     :long
@@ -6266,7 +6718,7 @@
      (xdoc::p
       "This completes the job started by @(tsee parse-logical-and-expression);
        it is analogous to @(tsee parse-expression-rest)."))
-    (b* (((reterr) (irr-expr) (irr-span) (irr-parstate))
+    (b* (((reterr) (irr-expr) (irr-span) parstate)
          ;; prev-expr
          ((erp token & parstate) (read-token parstate))
          ((when (not (token-punctuatorp token "&&"))) ; prev-expr not&&
@@ -6289,7 +6741,10 @@
   ;;;;;;;;;;;;;;;;;;;;;;;;;;;;;;;;;;;;;;;;
 
   (define parse-inclusive-or-expression ((parstate parstatep))
-    :returns (mv erp (expr exprp) (span spanp) (new-parstate parstatep))
+    :returns (mv erp
+                 (expr exprp)
+                 (span spanp)
+                 (new-parstate parstatep :hyp (parstatep parstate)))
     :parents (parser parse-exprs/decls)
     :short "Parse an inclusive disjunction expression."
     :long
@@ -6298,7 +6753,7 @@
       "We handle the left recursion in the grammar rule
        in the same way as for expressions:
        see @(tsee parse-expression)."))
-    (b* (((reterr) (irr-expr) (irr-span) (irr-parstate))
+    (b* (((reterr) (irr-expr) (irr-span) parstate)
          (psize (parsize parstate))
          ((erp expr span parstate) (parse-exclusive-or-expression parstate))
          ((unless (mbt (<= (parsize parstate) (1- psize))))
@@ -6311,7 +6766,10 @@
   (define parse-inclusive-or-expression-rest ((prev-expr exprp)
                                               (prev-span spanp)
                                               (parstate parstatep))
-    :returns (mv erp (expr exprp) (span spanp) (new-parstate parstatep))
+    :returns (mv erp
+                 (expr exprp)
+                 (span spanp)
+                 (new-parstate parstatep :hyp (parstatep parstate)))
     :parents (parser parse-exprs/decls)
     :short "Parse the rest of an inclusive disjunction expression."
     :long
@@ -6319,7 +6777,7 @@
      (xdoc::p
       "This completes the job started by @(tsee parse-inclusive-or-expression);
        it is analogous to @(tsee parse-expression-rest)."))
-    (b* (((reterr) (irr-expr) (irr-span) (irr-parstate))
+    (b* (((reterr) (irr-expr) (irr-span) parstate)
          ;; prev-expr
          ((erp token & parstate) (read-token parstate))
          ((when (not (token-punctuatorp token "|"))) ; prev-expr not|
@@ -6342,7 +6800,10 @@
   ;;;;;;;;;;;;;;;;;;;;;;;;;;;;;;;;;;;;;;;;
 
   (define parse-exclusive-or-expression ((parstate parstatep))
-    :returns (mv erp (expr exprp) (span spanp) (new-parstate parstatep))
+    :returns (mv erp
+                 (expr exprp)
+                 (span spanp)
+                 (new-parstate parstatep :hyp (parstatep parstate)))
     :parents (parser parse-exprs/decls)
     :short "Parse an exclusive disjunction expression."
     :long
@@ -6351,7 +6812,7 @@
       "We handle the left recursion in the grammar rule
        in the same way as for expressions:
        see @(tsee parse-expression)."))
-    (b* (((reterr) (irr-expr) (irr-span) (irr-parstate))
+    (b* (((reterr) (irr-expr) (irr-span) parstate)
          (psize (parsize parstate))
          ((erp expr span parstate) (parse-and-expression parstate))
          ((unless (mbt (<= (parsize parstate) (1- psize))))
@@ -6364,7 +6825,10 @@
   (define parse-exclusive-or-expression-rest ((prev-expr exprp)
                                               (prev-span spanp)
                                               (parstate parstatep))
-    :returns (mv erp (expr exprp) (span spanp) (new-parstate parstatep))
+    :returns (mv erp
+                 (expr exprp)
+                 (span spanp)
+                 (new-parstate parstatep :hyp (parstatep parstate)))
     :parents (parser parse-exprs/decls)
     :short "Parse the rest of an exclusive disjunction expression."
     :long
@@ -6372,7 +6836,7 @@
      (xdoc::p
       "This completes the job started by @(tsee parse-exclusive-or-expression);
        it is analogous to @(tsee parse-expression-rest)."))
-    (b* (((reterr) (irr-expr) (irr-span) (irr-parstate))
+    (b* (((reterr) (irr-expr) (irr-span) parstate)
          ;; prev-expr
          ((erp token & parstate) (read-token parstate))
          ((when (not (token-punctuatorp token "^"))) ; prev-expr not^
@@ -6394,7 +6858,10 @@
   ;;;;;;;;;;;;;;;;;;;;;;;;;;;;;;;;;;;;;;;;
 
   (define parse-and-expression ((parstate parstatep))
-    :returns (mv erp (expr exprp) (span spanp) (new-parstate parstatep))
+    :returns (mv erp
+                 (expr exprp)
+                 (span spanp)
+                 (new-parstate parstatep :hyp (parstatep parstate)))
     :parents (parser parse-exprs/decls)
     :short "Parse a conjunction expression."
     :long
@@ -6403,7 +6870,7 @@
       "We handle the left recursion in the grammar rule
        in the same way as for expressions:
        see @(tsee parse-expression)."))
-    (b* (((reterr) (irr-expr) (irr-span) (irr-parstate))
+    (b* (((reterr) (irr-expr) (irr-span) parstate)
          (psize (parsize parstate))
          ((erp expr span parstate) (parse-equality-expression parstate))
          ((unless (mbt (<= (parsize parstate) (1- psize))))
@@ -6416,7 +6883,10 @@
   (define parse-and-expression-rest ((prev-expr exprp)
                                      (prev-span spanp)
                                      (parstate parstatep))
-    :returns (mv erp (expr exprp) (span spanp) (new-parstate parstatep))
+    :returns (mv erp
+                 (expr exprp)
+                 (span spanp)
+                 (new-parstate parstatep :hyp (parstatep parstate)))
     :parents (parser parse-exprs/decls)
     :short "Parse the rest of a conjunction expression."
     :long
@@ -6424,7 +6894,7 @@
      (xdoc::p
       "This completes the job started by @(tsee parse-and-expression);
        it is analogous to @(tsee parse-expression-rest)."))
-    (b* (((reterr) (irr-expr) (irr-span) (irr-parstate))
+    (b* (((reterr) (irr-expr) (irr-span) parstate)
          ;; prev-expr
          ((erp token & parstate) (read-token parstate))
          ((when (not (token-punctuatorp token "&"))) ; prev-expr not&
@@ -6447,7 +6917,10 @@
   ;;;;;;;;;;;;;;;;;;;;;;;;;;;;;;;;;;;;;;;;
 
   (define parse-equality-expression ((parstate parstatep))
-    :returns (mv erp (expr exprp) (span spanp) (new-parstate parstatep))
+    :returns (mv erp
+                 (expr exprp)
+                 (span spanp)
+                 (new-parstate parstatep :hyp (parstatep parstate)))
     :parents (parser parse-exprs/decls)
     :short "Parse an equality expression."
     :long
@@ -6456,7 +6929,7 @@
       "We handle the left recursion in the grammar rule
        in the same way as for expressions:
        see @(tsee parse-expression)."))
-    (b* (((reterr) (irr-expr) (irr-span) (irr-parstate))
+    (b* (((reterr) (irr-expr) (irr-span) parstate)
          (psize (parsize parstate))
          ((erp expr span parstate) (parse-relational-expression parstate))
          ((unless (mbt (<= (parsize parstate) (1- psize))))
@@ -6469,7 +6942,10 @@
   (define parse-equality-expression-rest ((prev-expr exprp)
                                           (prev-span spanp)
                                           (parstate parstatep))
-    :returns (mv erp (expr exprp) (span spanp) (new-parstate parstatep))
+    :returns (mv erp
+                 (expr exprp)
+                 (span spanp)
+                 (new-parstate parstatep :hyp (parstatep parstate)))
     :parents (parser parse-exprs/decls)
     :short "Parse the rest of an equality expression."
     :long
@@ -6477,7 +6953,7 @@
      (xdoc::p
       "This completes the job started by @(tsee parse-equality-expression);
        it is analogous to @(tsee parse-expression-rest)."))
-    (b* (((reterr) (irr-expr) (irr-span) (irr-parstate))
+    (b* (((reterr) (irr-expr) (irr-span) parstate)
          ;; prev-expr
          ((erp token & parstate) (read-token parstate))
          ((when (not (token-equality-operator-p token))) ; prev-expr not-eqop
@@ -6501,7 +6977,10 @@
   ;;;;;;;;;;;;;;;;;;;;;;;;;;;;;;;;;;;;;;;;
 
   (define parse-relational-expression ((parstate parstatep))
-    :returns (mv erp (expr exprp) (span spanp) (new-parstate parstatep))
+    :returns (mv erp
+                 (expr exprp)
+                 (span spanp)
+                 (new-parstate parstatep :hyp (parstatep parstate)))
     :parents (parser parse-exprs/decls)
     :short "Parse a relational expression."
     :long
@@ -6510,7 +6989,7 @@
       "We handle the left recursion in the grammar rule
        in the same way as for expressions:
        see @(tsee parse-expression)."))
-    (b* (((reterr) (irr-expr) (irr-span) (irr-parstate))
+    (b* (((reterr) (irr-expr) (irr-span) parstate)
          (psize (parsize parstate))
          ((erp expr span parstate) (parse-shift-expression parstate))
          ((unless (mbt (<= (parsize parstate) (1- psize))))
@@ -6523,7 +7002,10 @@
   (define parse-relational-expression-rest ((prev-expr exprp)
                                             (prev-span spanp)
                                             (parstate parstatep))
-    :returns (mv erp (expr exprp) (span spanp) (new-parstate parstatep))
+    :returns (mv erp
+                 (expr exprp)
+                 (span spanp)
+                 (new-parstate parstatep :hyp (parstatep parstate)))
     :parents (parser parse-exprs/decls)
     :short "Parse the rest of a relational expression."
     :long
@@ -6531,7 +7013,7 @@
      (xdoc::p
       "This completes the job started by @(tsee parse-relational-expression);
        it is analogous to @(tsee parse-expression-rest)."))
-    (b* (((reterr) (irr-expr) (irr-span) (irr-parstate))
+    (b* (((reterr) (irr-expr) (irr-span) parstate)
          ;; prev-expr
          ((erp token & parstate) (read-token parstate))
          ((when (not (token-relational-operator-p token))) ; prev-expr not-relop
@@ -6554,7 +7036,10 @@
   ;;;;;;;;;;;;;;;;;;;;;;;;;;;;;;;;;;;;;;;;
 
   (define parse-shift-expression ((parstate parstatep))
-    :returns (mv erp (expr exprp) (span spanp) (new-parstate parstatep))
+    :returns (mv erp
+                 (expr exprp)
+                 (span spanp)
+                 (new-parstate parstatep :hyp (parstatep parstate)))
     :parents (parser parse-exprs/decls)
     :short "Parse a shift expression."
     :long
@@ -6563,7 +7048,7 @@
       "We handle the left recursion in the grammar rule
        in the same way as for expressions:
        see @(tsee parse-expression)."))
-    (b* (((reterr) (irr-expr) (irr-span) (irr-parstate))
+    (b* (((reterr) (irr-expr) (irr-span) parstate)
          (psize (parsize parstate))
          ((erp expr span parstate) (parse-additive-expression parstate))
          ((unless (mbt (<= (parsize parstate) (1- psize))))
@@ -6576,7 +7061,10 @@
   (define parse-shift-expression-rest ((prev-expr exprp)
                                        (prev-span spanp)
                                        (parstate parstatep))
-    :returns (mv erp (expr exprp) (span spanp) (new-parstate parstatep))
+    :returns (mv erp
+                 (expr exprp)
+                 (span spanp)
+                 (new-parstate parstatep :hyp (parstatep parstate)))
     :parents (parser parse-exprs/decls)
     :short "Parse the rest of a shift expression."
     :long
@@ -6584,7 +7072,7 @@
      (xdoc::p
       "This completes the job started by @(tsee parse-shift-expression);
        it is analogous to @(tsee parse-expression-rest)."))
-    (b* (((reterr) (irr-expr) (irr-span) (irr-parstate))
+    (b* (((reterr) (irr-expr) (irr-span) parstate)
          ;; prev-expr
          ((erp token & parstate) (read-token parstate))
          ((when (not (token-shift-operator-p token))) ; prev-expr not-shiftop
@@ -6607,7 +7095,10 @@
   ;;;;;;;;;;;;;;;;;;;;;;;;;;;;;;;;;;;;;;;;
 
   (define parse-additive-expression ((parstate parstatep))
-    :returns (mv erp (expr exprp) (span spanp) (new-parstate parstatep))
+    :returns (mv erp
+                 (expr exprp)
+                 (span spanp)
+                 (new-parstate parstatep :hyp (parstatep parstate)))
     :parents (parser parse-exprs/decls)
     :short "Parse an additive expression."
     :long
@@ -6616,7 +7107,7 @@
       "We handle the left recursion in the grammar rule
        in the same way as for expressions:
        see @(tsee parse-expression)."))
-    (b* (((reterr) (irr-expr) (irr-span) (irr-parstate))
+    (b* (((reterr) (irr-expr) (irr-span) parstate)
          (psize (parsize parstate))
          ((erp expr span parstate) (parse-multiplicative-expression parstate))
          ((unless (mbt (<= (parsize parstate) (1- psize))))
@@ -6629,7 +7120,10 @@
   (define parse-additive-expression-rest ((prev-expr exprp)
                                           (prev-span spanp)
                                           (parstate parstatep))
-    :returns (mv erp (expr exprp) (span spanp) (new-parstate parstatep))
+    :returns (mv erp
+                 (expr exprp)
+                 (span spanp)
+                 (new-parstate parstatep :hyp (parstatep parstate)))
     :parents (parser parse-exprs/decls)
     :short "Parse the rest of an additive expression."
     :long
@@ -6637,7 +7131,7 @@
      (xdoc::p
       "This completes the job started by @(tsee parse-additive-expression);
        it is analogous to @(tsee parse-expression-rest)."))
-    (b* (((reterr) (irr-expr) (irr-span) (irr-parstate))
+    (b* (((reterr) (irr-expr) (irr-span) parstate)
          ;; prev-expr
          ((erp token & parstate) (read-token parstate))
          ((when (not (token-additive-operator-p token))) ; prev-expr notaddop
@@ -6660,7 +7154,10 @@
   ;;;;;;;;;;;;;;;;;;;;;;;;;;;;;;;;;;;;;;;;
 
   (define parse-multiplicative-expression ((parstate parstatep))
-    :returns (mv erp (expr exprp) (span spanp) (new-parstate parstatep))
+    :returns (mv erp
+                 (expr exprp)
+                 (span spanp)
+                 (new-parstate parstatep :hyp (parstatep parstate)))
     :parents (parser parse-exprs/decls)
     :short "Parse a multiplicative expression."
     :long
@@ -6669,7 +7166,7 @@
       "We handle the left recursion in the grammar rule
        in the same way as for expressions:
        see @(tsee parse-expression)."))
-    (b* (((reterr) (irr-expr) (irr-span) (irr-parstate))
+    (b* (((reterr) (irr-expr) (irr-span) parstate)
          (psize (parsize parstate))
          ((erp expr span parstate) (parse-cast-expression parstate))
          ((unless (mbt (<= (parsize parstate) (1- psize))))
@@ -6682,7 +7179,10 @@
   (define parse-multiplicative-expression-rest ((prev-expr exprp)
                                                 (prev-span spanp)
                                                 (parstate parstatep))
-    :returns (mv erp (expr exprp) (span spanp) (new-parstate parstatep))
+    :returns (mv erp
+                 (expr exprp)
+                 (span spanp)
+                 (new-parstate parstatep :hyp (parstatep parstate)))
     :parents (parser parse-exprs/decls)
     :short "Parse the rest of a multiplicative expression."
     :long
@@ -6691,7 +7191,7 @@
       "This completes the job started by
        @(tsee parse-multiplicative-expression);
        it is analogous to @(tsee parse-expression-rest)."))
-    (b* (((reterr) (irr-expr) (irr-span) (irr-parstate))
+    (b* (((reterr) (irr-expr) (irr-span) parstate)
          ;; prev-expr
          ((erp token & parstate) (read-token parstate))
          ((when (not
@@ -6715,7 +7215,10 @@
   ;;;;;;;;;;;;;;;;;;;;;;;;;;;;;;;;;;;;;;;;
 
   (define parse-cast-expression ((parstate parstatep))
-    :returns (mv erp (expr exprp) (span spanp) (new-parstate parstatep))
+    :returns (mv erp
+                 (expr exprp)
+                 (span spanp)
+                 (new-parstate parstatep :hyp (parstatep parstate)))
     :parents (parser parse-exprs/decls)
     :short "Parse a cast expression."
     :long
@@ -6878,7 +7381,7 @@
         in parenthesis.
         We put back the token (if present),
         and we return the parenthesized expression.")))
-    (b* (((reterr) (irr-expr) (irr-span) (irr-parstate))
+    (b* (((reterr) (irr-expr) (irr-span) parstate)
          ((erp token span parstate) (read-token parstate)))
       (cond
        ;; If token is an open parenthesis,
@@ -6949,7 +7452,7 @@
                  ;; no larger than the initial one,
                  ;; so we just return the empty parser state.
                  ;; This is just logical: execution stops at the RAISE above.
-                 (b* ((parstate (init-parstate nil nil)))
+                 (b* ((parstate (init-parstate nil nil parstate)))
                    (reterr t)))
                 (parstate (unread-token parstate))) ;
              (parse-postfix-expression parstate))
@@ -7107,7 +7610,7 @@
                      ;; so we just return the empty parser state.
                      ;; This is just logical:
                      ;; execution stops at the RAISE above.
-                     (b* ((parstate (init-parstate nil nil)))
+                     (b* ((parstate (init-parstate nil nil parstate)))
                        (reterr t)))
                     (parstate (unread-token parstate))) ;
                  (parse-postfix-expression parstate))))))))
@@ -7124,7 +7627,10 @@
   ;;;;;;;;;;;;;;;;;;;;;;;;;;;;;;;;;;;;;;;;
 
   (define parse-unary-expression ((parstate parstatep))
-    :returns (mv erp (expr exprp) (span spanp) (new-parstate parstatep))
+    :returns (mv erp
+                 (expr exprp)
+                 (span spanp)
+                 (new-parstate parstatep :hyp (parstatep parstate)))
     :parents (parser parse-exprs/decls)
     :short "Parse a unary expression."
     :long
@@ -7141,7 +7647,7 @@
        we parse an expression or type name via a separate function,
        and based on the result we return a @('sizeof') expression with
        an expression, a type name, or an ambiguous type name or expression."))
-    (b* (((reterr) (irr-expr) (irr-span) (irr-parstate))
+    (b* (((reterr) (irr-expr) (irr-span) parstate)
          ((erp token span parstate) (read-token parstate)))
       (cond
        ;; If token may start a postfix expression
@@ -7249,7 +7755,10 @@
   ;;;;;;;;;;;;;;;;;;;;;;;;;;;;;;;;;;;;;;;;
 
   (define parse-postfix-expression ((parstate parstatep))
-    :returns (mv erp (expr exprp) (span spanp) (new-parstate parstatep))
+    :returns (mv erp
+                 (expr exprp)
+                 (span spanp)
+                 (new-parstate parstatep :hyp (parstatep parstate)))
     :parents (parser parse-exprs/decls)
     :short "Parse a postfix expression."
     :long
@@ -7339,7 +7848,7 @@
       (xdoc::li
        "If this fourth token is none of the above,
         we have an error.")))
-    (b* (((reterr) (irr-expr) (irr-span) (irr-parstate))
+    (b* (((reterr) (irr-expr) (irr-span) parstate)
          ((erp token span parstate) (read-token parstate)))
       (cond
        ;; If token is an open parenthesis,
@@ -7420,7 +7929,10 @@
   (define parse-postfix-expression-rest ((prev-expr exprp)
                                          (prev-span spanp)
                                          (parstate parstatep))
-    :returns (mv erp (expr exprp) (span spanp) (new-parstate parstatep))
+    :returns (mv erp
+                 (expr exprp)
+                 (span spanp)
+                 (new-parstate parstatep :hyp (parstatep parstate)))
     :parents (parser parse-exprs/decls)
     :short "Parse the rest of a postfix expression."
     :long
@@ -7446,7 +7958,7 @@
        as implied by the grammar.
        The recursion ends when the next token
        is absent or cannot start a postfix construct."))
-    (b* (((reterr) (irr-expr) (irr-span) (irr-parstate))
+    (b* (((reterr) (irr-expr) (irr-span) parstate)
          ;; prev-expr
          ((erp token span parstate) (read-token parstate)))
       (cond
@@ -7506,7 +8018,10 @@
   ;;;;;;;;;;;;;;;;;;;;;;;;;;;;;;;;;;;;;;;;
 
   (define parse-argument-expressions ((parstate parstatep))
-    :returns (mv erp (exprs expr-listp) (span spanp) (new-parstate parstatep))
+    :returns (mv erp
+                 (exprs expr-listp)
+                 (span spanp)
+                 (new-parstate parstatep :hyp (parstatep parstate)))
     :parents (parser parse-exprs/decls)
     :short "Parse zero or more argument expressions."
     :long
@@ -7530,7 +8045,7 @@
        and then we call a separate function
        to parse any additional arguments.
        Otherwise, we return the empty list of argument expressions."))
-    (b* (((reterr) nil (irr-span) (irr-parstate))
+    (b* (((reterr) nil (irr-span) parstate)
          ((erp token & parstate) (read-token parstate)))
       (cond
        ((token-expression-start-p token) ; expr...
@@ -7553,7 +8068,10 @@
   (define parse-argument-expressions-rest ((prev-exprs expr-listp)
                                            (prev-span spanp)
                                            (parstate parstatep))
-    :returns (mv erp (exprs expr-listp) (span spanp) (new-parstate parstatep))
+    :returns (mv erp
+                 (exprs expr-listp)
+                 (span spanp)
+                 (new-parstate parstatep :hyp (parstatep parstate)))
     :parents (parser parse-exprs/decls)
     :short "Parse the rest of one or more argument expressions."
     :long
@@ -7570,7 +8088,7 @@
       "We could extend the list in reverse (via @(tsee cons)),
        and then reverse it in the caller,
        but it probably does not make a big difference in performance."))
-    (b* (((reterr) nil (irr-span) (irr-parstate))
+    (b* (((reterr) nil (irr-span) parstate)
          ;; prev-exprs
          ((erp token & parstate) (read-token parstate))
          ((when (not (token-punctuatorp token ",")))
@@ -7592,7 +8110,10 @@
   ;;;;;;;;;;;;;;;;;;;;;;;;;;;;;;;;;;;;;;;;
 
   (define parse-primary-expression ((parstate parstatep))
-    :returns (mv erp (expr exprp) (span spanp) (new-parstate parstatep))
+    :returns (mv erp
+                 (expr exprp)
+                 (span spanp)
+                 (new-parstate parstatep :hyp (parstatep parstate)))
     :parents (parser parse-exprs/decls)
     :short "Parse a primary expression."
     :long
@@ -7620,7 +8141,7 @@
       "If the token is none of the above,
        including the token being absent,
        it is an error."))
-    (b* (((reterr) (irr-expr) (irr-span) (irr-parstate))
+    (b* (((reterr) (irr-expr) (irr-span) parstate)
          ((erp token span parstate) (read-token parstate)))
       (cond
        ((and token (token-case token :ident)) ; identifier
@@ -7683,7 +8204,7 @@
     :returns (mv erp
                  (genassocs genassoc-listp)
                  (span spanp)
-                 (new-parstate parstatep))
+                 (new-parstate parstatep :hyp (parstatep parstate)))
     :parents (parser parse-exprs/decls)
     :short "Parse zero or more reamaining generic associations."
     :long
@@ -7700,7 +8221,7 @@
        the list of generic expressions parsed so far,
        along with their span.
        This makes it easier to handle the span calculation."))
-    (b* (((reterr) nil (irr-span) (irr-parstate))
+    (b* (((reterr) nil (irr-span) parstate)
          ((erp token & parstate) (read-token parstate))
          ((when (not (token-punctuatorp token ",")))
           (b* ((parstate (if token (unread-token parstate) parstate)))
@@ -7721,7 +8242,10 @@
   ;;;;;;;;;;;;;;;;;;;;;;;;;;;;;;;;;;;;;;;;
 
   (define parse-generic-association ((parstate parstatep))
-    :returns (mv erp (genassoc genassocp) (span spanp) (new-parstate parstatep))
+    :returns (mv erp
+                 (genassoc genassocp)
+                 (span spanp)
+                 (new-parstate parstatep :hyp (parstatep parstate)))
     :parents (parser parse-exprs/decls)
     :short "Parse a generic association."
     :long
@@ -7737,7 +8261,7 @@
        we parse a colon and an assignment expression.")
      (xdoc::p
       "If the token is none of the above, it is an error."))
-    (b* (((reterr) (irr-genassoc) (irr-span) (irr-parstate))
+    (b* (((reterr) (irr-genassoc) (irr-span) parstate)
          ((erp token span parstate) (read-token parstate)))
       (cond
        ((token-type-name-start-p token) ; typename...
@@ -7792,7 +8316,10 @@
   (define parse-compound-literal ((tyname tynamep)
                                   (first-span spanp)
                                   (parstate parstatep))
-    :returns (mv erp (expr exprp) (span spanp) (new-parstate parstatep))
+    :returns (mv erp
+                 (expr exprp)
+                 (span spanp)
+                 (new-parstate parstatep :hyp (parstatep parstate)))
     :parents (parser parse-exprs/decls)
     :short "Parse a compound literal."
     :long
@@ -7802,7 +8329,7 @@
        So we start by parsing an open curly brace,
        a list of initializers,
        and a closed curly brace."))
-    (b* (((reterr) (irr-expr) (irr-span) (irr-parstate))
+    (b* (((reterr) (irr-expr) (irr-span) parstate)
          ((erp & parstate) (read-punctuator "{" parstate)) ; {
          ((erp desiniters final-comma & parstate) ; { inits [,]
           (parse-initializer-list parstate))
@@ -7818,7 +8345,10 @@
   ;;;;;;;;;;;;;;;;;;;;;;;;;;;;;;;;;;;;;;;;
 
   (define parse-constant-expression ((parstate parstatep))
-    :returns (mv erp (cexpr const-exprp) (span spanp) (new-parstate parstatep))
+    :returns (mv erp
+                 (cexpr const-exprp)
+                 (span spanp)
+                 (new-parstate parstatep :hyp (parstatep parstate)))
     :parents (parser parse-exprs/decls)
     :short "Parse a constant expression."
     :long
@@ -7833,7 +8363,7 @@
        just as a wrapper of an expression;
        the wrapper marks the expression as intended to be in fact constant,
        but the check that that is the case is done elsewhere."))
-    (b* (((reterr) (irr-const-expr) (irr-span) (irr-parstate))
+    (b* (((reterr) (irr-const-expr) (irr-span) parstate)
          ((erp expr span parstate) (parse-conditional-expression parstate)))
       (retok (const-expr expr) span parstate))
     :measure (two-nats-measure (parsize parstate) 17))
@@ -7845,7 +8375,7 @@
     :returns (mv erp
                  (statassert statassertp)
                  (span spanp)
-                 (new-parstate parstatep))
+                 (new-parstate parstatep :hyp (parstatep parstate)))
     :parents (parser parse-exprs/decls)
     :short "Parse a static assert declaration."
     :long
@@ -7860,7 +8390,7 @@
       "We read the remaining components of the grammar rule,
        one after the other.
        There are no alternatives."))
-    (b* (((reterr) (irr-statassert) (irr-span) (irr-parstate))
+    (b* (((reterr) (irr-statassert) (irr-span) parstate)
          ((erp & parstate) (read-punctuator "(" parstate))
          ((erp cexpr & parstate) (parse-constant-expression parstate))
          ((erp & parstate) (read-punctuator "," parstate))
@@ -7876,7 +8406,10 @@
   ;;;;;;;;;;;;;;;;;;;;;;;;;;;;;;;;;;;;;;;;
 
   (define parse-designator ((parstate parstatep))
-    :returns (mv erp (designor designorp) (span spanp) (new-parstate parstatep))
+    :returns (mv erp
+                 (designor designorp)
+                 (span spanp)
+                 (new-parstate parstatep :hyp (parstatep parstate)))
     :parents (parser parse-exprs/decls)
     :short "Parse a designator."
     :long
@@ -7884,7 +8417,7 @@
      (xdoc::p
       "There are two kinds of designators,
        easily distinguished by their first token."))
-    (b* (((reterr) (irr-designor) (irr-span) (irr-parstate))
+    (b* (((reterr) (irr-designor) (irr-span) parstate)
          ((erp token span parstate) (read-token parstate)))
       (cond
        ((token-punctuatorp token "[") ; [
@@ -7907,7 +8440,7 @@
     :returns (mv erp
                  (designors designor-listp)
                  (span spanp)
-                 (new-parstate parstatep))
+                 (new-parstate parstatep :hyp (parstatep parstate)))
     :parents (parser parse-exprs/decls)
     :short "Parse a designator list."
     :long
@@ -7923,7 +8456,7 @@
        where it is followed by an equal sign.
        So there is no overlap between the equal sign
        and the possible starts of a designator."))
-    (b* (((reterr) nil (irr-span) (irr-parstate))
+    (b* (((reterr) nil (irr-span) parstate)
          (psize (parsize parstate))
          ((erp designor span parstate) (parse-designator parstate)) ; designor
          ((unless (mbt (<= (parsize parstate) (1- psize))))
@@ -7946,7 +8479,10 @@
   ;;;;;;;;;;;;;;;;;;;;;;;;;;;;;;;;;;;;;;;;
 
   (define parse-initializer ((parstate parstatep))
-    :returns (mv erp (initer initerp) (span spanp) (new-parstate parstatep))
+    :returns (mv erp
+                 (initer initerp)
+                 (span spanp)
+                 (new-parstate parstatep :hyp (parstatep parstate)))
     :parents (parser parse-exprs/decls)
     :short "Parse an initializer."
     :long
@@ -7959,7 +8495,7 @@
        If the token is an open curly brace,
        we must have an aggregate initializer.
        There is no overlap between these two cases."))
-    (b* (((reterr) (irr-initer) (irr-span) (irr-parstate))
+    (b* (((reterr) (irr-initer) (irr-span) parstate)
          ((erp token span parstate) (read-token parstate)))
       (cond
        ((token-expression-start-p token) ; expr...
@@ -8006,7 +8542,7 @@
     :returns (mv erp
                  (desiniter desiniterp)
                  (span spanp)
-                 (new-parstate parstatep))
+                 (new-parstate parstatep :hyp (parstatep parstate)))
     :parents (parser parse-exprs/decls)
     :short "Parse an initializer with an optional designation."
     :long
@@ -8019,7 +8555,7 @@
        we parse an initializer.
        Note that there is no overlap between the starts of
        designations and initializers."))
-    (b* (((reterr) (irr-desiniter) (irr-span) (irr-parstate))
+    (b* (((reterr) (irr-desiniter) (irr-span) parstate)
          ((erp token span parstate) (read-token parstate)))
       (cond
        ((token-designation-start-p token) ; designation...
@@ -8075,7 +8611,7 @@
                  (desiniters desiniter-listp)
                  (final-comma booleanp)
                  (span spanp)
-                 (new-parstate parstatep))
+                 (new-parstate parstatep :hyp (parstatep parstate)))
     :parents (parser parse-exprs/decls)
     :short "Parse a list of one or more initializers."
     :long
@@ -8100,7 +8636,7 @@
        We parse that comma (if present) in this function.
        So, technically, this function parses slightly more then
        an @('initializer-list') as defined in the ABNF grammar."))
-    (b* (((reterr) nil nil (irr-span) (irr-parstate))
+    (b* (((reterr) nil nil (irr-span) parstate)
          (psize (parsize parstate))
          ((erp desiniter span parstate) ; initializer
           (parse-designation?-initializer parstate))
@@ -8186,10 +8722,13 @@
   ;;;;;;;;;;;;;;;;;;;;;;;;;;;;;;;;;;;;;;;;
 
   (define parse-enumerator ((parstate parstatep))
-    :returns (mv erp (enumer enumerp) (span spanp) (new-parstate parstatep))
+    :returns (mv erp
+                 (enumer enumerp)
+                 (span spanp)
+                 (new-parstate parstatep :hyp (parstatep parstate)))
     :parents (parser parse-exprs/decls)
     :short "Parse an enumerator."
-    (b* (((reterr) (irr-enumer) (irr-span) (irr-parstate))
+    (b* (((reterr) (irr-enumer) (irr-span) parstate)
          ;; An enumerator always starts with (or is) an identifier.
          ((erp ident span parstate) (read-identifier parstate)) ; ident
          ;; The identifier may be the whole enumerator, or there may be more,
@@ -8220,7 +8759,7 @@
                  (enumers enumer-listp)
                  (final-comma booleanp)
                  (span spanp)
-                 (new-parstate parstatep))
+                 (new-parstate parstatep :hyp (parstatep parstate)))
     :parents (parser parse-exprs/decls)
     :short "Parse a list of one or more enumerators."
     :long
@@ -8233,7 +8772,7 @@
      (xdoc::p
       "This function does not consume the closed curly brace.
        The caller must consume it."))
-    (b* (((reterr) nil nil (irr-span) (irr-parstate))
+    (b* (((reterr) nil nil (irr-span) parstate)
          ;; The list must not be empty, so we parse the first enumerator.
          (psize (parsize parstate))
          ((erp enumer enumer-span parstate)
@@ -8310,7 +8849,7 @@
     :returns (mv erp
                  (specqual spec/qual-p)
                  (span spanp)
-                 (new-parstate parstatep))
+                 (new-parstate parstatep :hyp (parstatep parstate)))
     :parents (parser parse-exprs/decls)
     :short "Parse a specifier or qualifier."
     :long
@@ -8351,7 +8890,7 @@
        the @('_Atomic') must start a type specifier,
        so we must parse a type name after the open parenthesis,
        and finally the closing parenthesis."))
-    (b* (((reterr) (irr-spec/qual) (irr-span) (irr-parstate))
+    (b* (((reterr) (irr-spec/qual) (irr-span) parstate)
          ((erp token span parstate) (read-token parstate)))
       (cond
        ;; If token is a type specifier consisting of a single keyword,
@@ -8490,7 +9029,7 @@
     :returns (mv erp
                  (specquals spec/qual-listp)
                  (span spanp)
-                 (new-parstate parstatep))
+                 (new-parstate parstatep :hyp (parstatep parstate)))
     :parents (parser parse-exprs/decls)
     :short "Parse a list of one or more specifiers and qualifiers."
     :long
@@ -8502,7 +9041,7 @@
        Lists of specifiers and qualifiers have the same restrictions
        as lists of declaration specifiers with respect to
        type specifiers, which we use to resolve identifier ambiguities."))
-    (b* (((reterr) nil (irr-span) (irr-parstate))
+    (b* (((reterr) nil (irr-span) parstate)
          (psize (parsize parstate))
          ((erp specqual first-span parstate) ; specqual
           (parse-specifier/qualifier tyspec-seenp parstate))
@@ -8561,7 +9100,10 @@
 
   (define parse-declaration-specifier ((tyspec-seenp booleanp)
                                        (parstate parstatep))
-    :returns (mv erp (declspec declspecp) (span spanp) (new-parstate parstatep))
+    :returns (mv erp
+                 (declspec declspecp)
+                 (span spanp)
+                 (new-parstate parstatep :hyp (parstatep parstate)))
     :parents (parser parse-exprs/decls)
     :short "Parse a declaration specifier."
     :long
@@ -8601,7 +9143,7 @@
        is resolved in the same way as in @(tsee parse-specifier/qualifier),
        which motivates the @('tyspec-seenp') flag passed to this function;
        see that function's documentation."))
-    (b* (((reterr) (irr-declspec) (irr-span) (irr-parstate))
+    (b* (((reterr) (irr-declspec) (irr-span) parstate)
          ((erp token span parstate) (read-token parstate)))
       (cond
        ;; If token is a storage class specifier,
@@ -8760,7 +9302,7 @@
     :returns (mv erp
                  (declspecs declspec-listp)
                  (span spanp)
-                 (new-parstate parstatep))
+                 (new-parstate parstatep :hyp (parstatep parstate)))
     :parents (parser parse-exprs/decls)
     :short "Parse a list of one or more declaration specifiers."
     :long
@@ -8796,7 +9338,7 @@
        the identifier cannot be (the start of) a declarator,
        because we have not found a type specifier yet,
        and thus the identifier must be the missing type specifier."))
-    (b* (((reterr) nil (irr-span) (irr-parstate))
+    (b* (((reterr) nil (irr-span) parstate)
          (psize (parsize parstate))
          ((erp declspec first-span parstate) ; declspec
           (parse-declaration-specifier tyspec-seenp parstate))
@@ -8857,7 +9399,7 @@
     :returns (mv erp
                  (strunispec strunispecp)
                  (span spanp)
-                 (new-parstate parstatep))
+                 (new-parstate parstatep :hyp (parstatep parstate)))
     :parents (parser parse-exprs/decls)
     :short "Parse or structure or union specifier."
     :long
@@ -8870,7 +9412,7 @@
        whether it is a structure or a union,
        which is done in @(tsee type-spec) instead;
        this is how we have factored our abstract syntax."))
-    (b* (((reterr) (irr-strunispec) (irr-span) (irr-parstate))
+    (b* (((reterr) (irr-strunispec) (irr-span) parstate)
          ;; There must be at least one token (identifier of open curly brace),
          ;; so we read one.
          ((erp token span parstate) (read-token parstate)))
@@ -8930,7 +9472,10 @@
   ;;;;;;;;;;;;;;;;;;;;;;;;;;;;;;;;;;;;;;;;
 
   (define parse-enum-specifier ((first-span spanp) (parstate parstatep))
-    :returns (mv erp (enumspec enumspecp) (span spanp) (new-parstate parstatep))
+    :returns (mv erp
+                 (enumspec enumspecp)
+                 (span spanp)
+                 (new-parstate parstatep :hyp (parstatep parstate)))
     :parents (parser parse-exprs/decls)
     :short "Parse an enumeration specifier."
     :long
@@ -8939,7 +9484,7 @@
       "This is called after parsing the initial @('enum') keyword.")
      (xdoc::p
       "The span of the @('enum') keyword is passed as input here."))
-    (b* (((reterr) (irr-enumspec) (irr-span) (irr-parstate))
+    (b* (((reterr) (irr-enumspec) (irr-span) parstate)
          ;; There must be at least one token (identifier of open curly brace),
          ;; so we read one.
          ((erp token span parstate) (read-token parstate)))
@@ -9003,7 +9548,7 @@
     :returns (mv erp
                  (alignspec align-specp)
                  (span spanp)
-                 (new-parstate parstatep))
+                 (new-parstate parstatep :hyp (parstatep parstate)))
     :parents (parser parse-exprs/decls)
     :short "Parse an alignment specifier."
     :long
@@ -9012,7 +9557,7 @@
       "This is called after parsing the initial @('_Alignas') keyword.")
      (xdoc::p
       "The span of the @('_Alignas') keyword is passed as input here."))
-    (b* (((reterr) (irr-align-spec) (irr-span) (irr-parstate))
+    (b* (((reterr) (irr-align-spec) (irr-span) parstate)
          ;; There must be an open parenthesis.
          ((erp & parstate) (read-punctuator "(" parstate)) ; (
          ;; Next comes a possibly ambiguous expression or type name.
@@ -9046,7 +9591,7 @@
     :returns (mv erp
                  (dirabsdeclor dirabsdeclorp)
                  (span spanp)
-                 (new-parstate parstatep))
+                 (new-parstate parstatep :hyp (parstatep parstate)))
     :parents (parser parse-exprs/decls)
     :short "Parse an array or function abstract declarator."
     :long
@@ -9057,7 +9602,7 @@
        See @(tsee parse-direct-abstract-declarator).")
      (xdoc::p
       "This function is called when we expect this kind of declarator."))
-    (b* (((reterr) (irr-dirabsdeclor) (irr-span) (irr-parstate))
+    (b* (((reterr) (irr-dirabsdeclor) (irr-span) parstate)
          ((erp token span parstate) (read-token parstate)))
       (cond
        ;; If token is an open square bracket,
@@ -9242,7 +9787,7 @@
     :returns (mv erp
                  (dirabsdeclor dirabsdeclorp)
                  (span spanp)
-                 (new-parstate parstatep))
+                 (new-parstate parstatep :hyp (parstatep parstate)))
     :parents (parser parse-exprs/decls)
     :short "Parse a direct abstract declarator."
     :long
@@ -9263,7 +9808,7 @@
        or a parenthesized abstract declarator
        followed by a sequence of
        zero or more array and function abstract declarators."))
-    (b* (((reterr) (irr-dirabsdeclor) (irr-span) (irr-parstate))
+    (b* (((reterr) (irr-dirabsdeclor) (irr-span) parstate)
          ((erp token span parstate) (read-token parstate)))
       (cond
        ;; If token is an open parenthesis,
@@ -9350,7 +9895,7 @@
     :returns (mv erp
                  (dirabsdeclor dirabsdeclorp)
                  (span spanp)
-                 (new-parstate parstatep))
+                 (new-parstate parstatep :hyp (parstatep parstate)))
     :parents (parser parse-exprs/decls)
     :short "Parse the rest of a direct abstract declartor."
     :long
@@ -9363,7 +9908,7 @@
        and in this function we read zero or more
        additional array and function abstract declarators,
        combining them with the one passed to this function."))
-    (b* (((reterr) (irr-dirabsdeclor) (irr-span) (irr-parstate))
+    (b* (((reterr) (irr-dirabsdeclor) (irr-span) parstate)
          ;; We read the next token, to determine whether
          ;; there is another array or function abstract declarator.
          ((erp token & parstate) (read-token parstate)))
@@ -9412,7 +9957,7 @@
     :returns (mv erp
                  (absdeclor absdeclorp)
                  (span spanp)
-                 (new-parstate parstatep))
+                 (new-parstate parstatep :hyp (parstatep parstate)))
     :parents (parser parse-exprs/decls)
     :short "Parse an abstract declarator."
     :long
@@ -9422,7 +9967,7 @@
        a pointer,
        or a direct abstract declarator,
        or a pointer followed by a direct abstract declarator."))
-    (b* (((reterr) (irr-absdeclor) (irr-span) (irr-parstate))
+    (b* (((reterr) (irr-absdeclor) (irr-span) parstate)
          ((erp token span parstate) (read-token parstate)))
       (cond
        ;; If token is a star, we must have a pointer,
@@ -9488,7 +10033,7 @@
     :returns (mv erp
                  (dirdeclor dirdeclorp)
                  (span spanp)
-                 (new-parstate parstatep))
+                 (new-parstate parstatep :hyp (parstatep parstate)))
     :parents (parser parse-exprs/decls)
     :short "Parse an array or function declarator."
     :long
@@ -9512,7 +10057,7 @@
        we always generate @(':function-params') during parsing,
        and potentially re-classify it to @(':function-names')
        during post-parsing semantic analysis."))
-    (b* (((reterr) (irr-dirdeclor) (irr-span) (irr-parstate))
+    (b* (((reterr) (irr-dirdeclor) (irr-span) parstate)
          ((erp token & parstate) (read-token parstate)))
       (cond
        ;; If token is an open square bracket,
@@ -9745,7 +10290,7 @@
     :returns (mv erp
                  (dirdeclor dirdeclorp)
                  (span spanp)
-                 (new-parstate parstatep))
+                 (new-parstate parstatep :hyp (parstatep parstate)))
     :parents (parser parse-exprs/decls)
     :short "Parse a direct declarator."
     :long
@@ -9758,7 +10303,7 @@
        First we parse the initial identifier or parenthesized declarator,
        then we call a separate function to parse
        the zero or more array or function constructs."))
-    (b* (((reterr) (irr-dirdeclor) (irr-span) (irr-parstate))
+    (b* (((reterr) (irr-dirdeclor) (irr-span) parstate)
          ((erp token span parstate) (read-token parstate)))
       (cond
        ;; If token is an identifier,
@@ -9797,7 +10342,7 @@
     :returns (mv erp
                  (dirdeclor dirdeclorp)
                  (span spanp)
-                 (new-parstate parstatep))
+                 (new-parstate parstatep :hyp (parstatep parstate)))
     :parents (parser parse-exprs/decls)
     :short "Parse the rest of a direct declarator."
     :long
@@ -9809,7 +10354,7 @@
        and which is a direct declarator itself,
        and is passed to this function as the @('prev-dirdeclor') input,
        along with its span."))
-    (b* (((reterr) (irr-dirdeclor) (irr-span) (irr-parstate))
+    (b* (((reterr) (irr-dirdeclor) (irr-span) parstate)
          ;; We read the next token, to determine whether
          ;; there is another array or function declarator.
          ((erp token & parstate) (read-token parstate)))
@@ -9848,7 +10393,10 @@
   ;;;;;;;;;;;;;;;;;;;;;;;;;;;;;;;;;;;;;;;;
 
   (define parse-declarator ((parstate parstatep))
-    :returns (mv erp (declor declorp) (span spanp) (new-parstate parstatep))
+    :returns (mv erp
+                 (declor declorp)
+                 (span spanp)
+                 (new-parstate parstatep :hyp (parstatep parstate)))
     :parents (parser parse-exprs/decls)
     :short "Parse a declarator."
     :long
@@ -9856,7 +10404,7 @@
      (xdoc::p
       "A declarator has an optional pointer part
        followed by a mandatory direct declarator."))
-    (b* (((reterr) (irr-declor) (irr-span) (irr-parstate))
+    (b* (((reterr) (irr-declor) (irr-span) parstate)
          ((erp token span parstate) (read-token parstate)))
       (cond
        ;; If token is a star, we must have a pointer,
@@ -9887,7 +10435,7 @@
     :returns (mv erp
                  (structdeclor structdeclorp)
                  (span spanp)
-                 (new-parstate parstatep))
+                 (new-parstate parstatep :hyp (parstatep parstate)))
     :parents (parser parse-exprs/decls)
     :short "Parse a structure declarator."
     :long
@@ -9897,7 +10445,7 @@
        a declarator,
        or a declarator followed by colon and a constant expression,
        or a colon and a constant expression."))
-    (b* (((reterr) (irr-structdeclor) (irr-span) (irr-parstate))
+    (b* (((reterr) (irr-structdeclor) (irr-span) parstate)
          ((erp token span parstate) (read-token parstate)))
       (cond
        ;; If token may start a declarator, we parse it,
@@ -9950,7 +10498,7 @@
     :returns (mv erp
                  (structdeclors structdeclor-listp)
                  (span spanp)
-                 (new-parstate parstatep))
+                 (new-parstate parstatep :hyp (parstatep parstate)))
     :parents (parser parse-exprs/decls)
     :short "Parse a list of one or more structure declarator."
     :long
@@ -9959,7 +10507,7 @@
       "We parse a structure declarator, which must be present.
        Then if we have a comma we recursively call this function
        to parse one or more structure declarators."))
-    (b* (((reterr) nil (irr-span) (irr-parstate))
+    (b* (((reterr) nil (irr-span) parstate)
          (psize (parsize parstate))
          ((erp structdeclor span parstate) ; structdeclor
           (parse-struct-declarator parstate))
@@ -9991,7 +10539,7 @@
     :returns (mv erp
                  (structdecl structdeclp)
                  (span spanp)
-                 (new-parstate parstatep))
+                 (new-parstate parstatep :hyp (parstatep parstate)))
     :parents (parser parse-exprs/decls)
     :short "Parse a structure declaration."
     :long
@@ -10005,7 +10553,7 @@
        a non-assert structure declaration
        may start with the @('__extension__') keyword,
        and may end (before the semicolon) with attribute specifiers."))
-    (b* (((reterr) (irr-structdecl) (irr-span) (irr-parstate))
+    (b* (((reterr) (irr-structdecl) (irr-span) parstate)
          ((erp token span parstate) (read-token parstate)))
       (cond
        ;; If token is the '_Static_assert' keyword,
@@ -10024,7 +10572,8 @@
               (if (and (token-keywordp token "__extension__")
                        (parstate->gcc parstate))
                   (mv t parstate)
-                (mv nil (if token (unread-token parstate) parstate))))
+                (b* ((parstate (if token (unread-token parstate) parstate)))
+                  (mv nil parstate))))
              ;; [__extension__]
              (psize (parsize parstate))
              ((erp specquals span parstate) ; [__extension__] specquals
@@ -10103,7 +10652,7 @@
     :returns (mv erp
                  (structdecls structdecl-listp)
                  (span spanp)
-                 (new-parstate parstatep))
+                 (new-parstate parstatep :hyp (parstatep parstate)))
     :parents (parser parse-exprs/decls)
     :short "Parse a list of one or more structure declarations."
     :long
@@ -10112,7 +10661,7 @@
       "We parse the first structure declaration, which must be present.
        Then we recursively call this function if the next token
        may start another structure declaration."))
-    (b* (((reterr) nil (irr-span) (irr-parstate))
+    (b* (((reterr) nil (irr-span) parstate)
          (psize (parsize parstate))
          ((erp structdecl span parstate) ; structdecl
           (parse-struct-declaration parstate))
@@ -10141,7 +10690,7 @@
     :returns (mv erp
                  (paramdecl paramdeclp)
                  (span spanp)
-                 (new-parstate parstatep))
+                 (new-parstate parstatep :hyp (parstatep parstate)))
     :parents (parser parse-exprs/decls)
     :short "Parse a parameter declaration."
     :long
@@ -10159,7 +10708,7 @@
        we parse a possibly ambiguous declarator or abstract declarator,
        and generate a parameter declarator accordingly,
        and then a parameter declaration with the declaration specifiers."))
-    (b* (((reterr) (irr-paramdecl) (irr-span) (irr-parstate))
+    (b* (((reterr) (irr-paramdecl) (irr-span) parstate)
          (psize (parsize parstate))
          ((erp declspecs span parstate) ; declspecs
           (parse-declaration-specifiers nil parstate))
@@ -10220,7 +10769,7 @@
                  (paramdecls paramdecl-listp)
                  (ellipsis booleanp)
                  (span spanp)
-                 (new-parstate parstatep))
+                 (new-parstate parstatep :hyp (parstatep parstate)))
     :parents (parser parse-exprs/decls)
     :short "Parse a list of one or more parameter declarations."
     :long
@@ -10232,7 +10781,7 @@
        So we must read a bit further to check that;
        if there may be indeed another parameter declaration,
        we recursively parse the remaining list of one or more."))
-    (b* (((reterr) nil nil (irr-span) (irr-parstate))
+    (b* (((reterr) nil nil (irr-span) parstate)
          (psize (parsize parstate))
          ((erp paramdecl span parstate) ; paramdecl
           (parse-parameter-declaration parstate))
@@ -10277,7 +10826,10 @@
   ;;;;;;;;;;;;;;;;;;;;;;;;;;;;;;;;;;;;;;;;
 
   (define parse-type-name ((parstate parstatep))
-    :returns (mv erp (tyname tynamep) (span spanp) (new-parstate parstatep))
+    :returns (mv erp
+                 (tyname tynamep)
+                 (span spanp)
+                 (new-parstate parstatep :hyp (parstatep parstate)))
     :parents (parser parse-exprs/decls)
     :short "Parse a type name."
     :long
@@ -10287,7 +10839,7 @@
        which may be followed by an abstract declarator.
        We parse the specifier and qualifier list,
        and then we parse the abstract declarator if present."))
-    (b* (((reterr) (irr-tyname) (irr-span) (irr-parstate))
+    (b* (((reterr) (irr-tyname) (irr-span) parstate)
          (psize (parsize parstate))
          ((erp specquals span parstate) ; specquals
           (parse-specifier-qualifier-list nil parstate))
@@ -10319,7 +10871,7 @@
     :returns (mv erp
                  (expr/tyname amb?-expr/tyname-p)
                  (span spanp)
-                 (new-parstate parstatep))
+                 (new-parstate parstatep :hyp (parstatep parstate)))
     :parents (parser parse-exprs/decls)
     :short "Parse an expression or a type name."
     :long
@@ -10357,7 +10909,7 @@
        should not exceed the size of the input before backtracking.
        For now we insert a run-time check without @(tsee mbt),
        but we plan to revisit this to see if we can have an @(tsee mbt)."))
-    (b* (((reterr) (irr-amb?-expr/tyname) (irr-span) (irr-parstate))
+    (b* (((reterr) (irr-amb?-expr/tyname) (irr-span) parstate)
          (parstate (record-checkpoint parstate)) ; we will backtrack here
          (psize (parsize parstate))
          ((mv erp-expr expr span-expr parstate) (parse-expression parstate)))
@@ -10375,7 +10927,7 @@
                 ;; no larger than the initial one,
                 ;; so we just return the empty parser state.
                 ;; This is just logical: execution stops at the RAISE above.
-                (b* ((parstate (init-parstate nil nil)))
+                (b* ((parstate (init-parstate nil nil parstate)))
                   (reterr t)))
                ((erp tyname span parstate) (parse-type-name parstate))
                ;; Ensure there is a closed parenthesis,
@@ -10406,7 +10958,7 @@
                     ;; so we just return the empty parser state.
                     ;; This is just logical:
                     ;; execution stops at the RAISE above.
-                    (b* ((parstate (init-parstate nil nil)))
+                    (b* ((parstate (init-parstate nil nil parstate)))
                       (reterr t)))
                    (parstate
                     (record-checkpoint parstate)) ; we may backtrack again
@@ -10434,7 +10986,7 @@
                           ;; so we just return the empty parser state.
                           ;; This is just logical:
                           ;; execution stops at the RAISE above.
-                          (b* ((parstate (init-parstate nil nil)))
+                          (b* ((parstate (init-parstate nil nil parstate)))
                             (reterr t)))
                          ((mv erp expr1 span-expr1 parstate)
                           (parse-expression parstate))
@@ -10504,7 +11056,7 @@
                             ;; so we just return the empty parser state.
                             ;; This is just logical:
                             ;; execution stops at the RAISE above.
-                            (b* ((parstate (init-parstate nil nil)))
+                            (b* ((parstate (init-parstate nil nil parstate)))
                               (reterr t)))
                            ((mv erp expr1 span-expr1 parstate)
                             (parse-expression parstate))
@@ -10546,7 +11098,7 @@
                   ;; no larger than the initial one,
                   ;; so we just return the empty parser state.
                   ;; This is just logical: execution stops at the RAISE above.
-                  (b* ((parstate (init-parstate nil nil)))
+                  (b* ((parstate (init-parstate nil nil parstate)))
                     (reterr t)))
                  ((erp tyname span parstate) (parse-type-name parstate))
                  ;; Ensure there is a closed parenthesis,
@@ -10562,7 +11114,7 @@
     :returns (mv erp
                  (declor/absdeclor amb?-declor/absdeclor-p)
                  (span spanp)
-                 (new-parstate parstatep))
+                 (new-parstate parstatep :hyp (parstatep parstate)))
     :parents (parser parse-exprs/decls)
     :short "Parse a declarator or an abstract declarator."
     :long
@@ -10595,7 +11147,7 @@
        we also ensure that the next token is a comma or closed parenthesis,
        otherwise we regard the parsing of the abstract declarator
        to have failed."))
-    (b* (((reterr) (irr-amb?-declor/absdeclor) (irr-span) (irr-parstate))
+    (b* (((reterr) (irr-amb?-declor/absdeclor) (irr-span) parstate)
          (parstate (record-checkpoint parstate)) ; we will backtrack here
          (psize (parsize parstate))
          ((mv erp-declor declor span-declor parstate)
@@ -10614,7 +11166,7 @@
                 ;; no larger than the initial one,
                 ;; so we just return the empty parser state.
                 ;; This is just logical: execution stops at the RAISE above.
-                (b* ((parstate (init-parstate nil nil)))
+                (b* ((parstate (init-parstate nil nil parstate)))
                   (reterr t)))
                ((erp absdeclor span parstate)
                 (parse-abstract-declarator parstate)))
@@ -10634,7 +11186,7 @@
               ;; so we just return the empty parser state.
               ;; This is just logical:
               ;; execution stops at the RAISE above.
-              (b* ((parstate (init-parstate nil nil)))
+              (b* ((parstate (init-parstate nil nil parstate)))
                 (reterr t)))
              (parstate (record-checkpoint parstate)) ; we may backtrack again
              ((mv erp absdeclor span-absdeclor parstate)
@@ -10661,7 +11213,7 @@
                     ;; so we just return the empty parser state.
                     ;; This is just logical:
                     ;; execution stops at the RAISE above.
-                    (b* ((parstate (init-parstate nil nil)))
+                    (b* ((parstate (init-parstate nil nil parstate)))
                       (reterr t)))
                    ((mv erp declor1 span-declor1 parstate)
                     (parse-declarator parstate))
@@ -10734,7 +11286,7 @@
                       ;; so we just return the empty parser state.
                       ;; This is just logical:
                       ;; execution stops at the RAISE above.
-                      (b* ((parstate (init-parstate nil nil)))
+                      (b* ((parstate (init-parstate nil nil parstate)))
                         (reterr t)))
                      ((mv erp declor1 span-declor1 parstate)
                       (parse-declarator parstate))
@@ -10767,7 +11319,7 @@
     :returns (mv erp
                  (attrparams expr-listp)
                  (span spanp)
-                 (new-parstate parstatep))
+                 (new-parstate parstatep :hyp (parstatep parstate)))
     :parents (parser parse-exprs/decls)
     :short "Parse attribute parameters."
     :long
@@ -10781,7 +11333,7 @@
        We re-use @(tsee parse-argument-expressions)
        to parse the zero or more comma-separated expressions.
        This parsing function does exactly what is needed here."))
-    (b* (((reterr) nil (irr-span) (irr-parstate))
+    (b* (((reterr) nil (irr-span) parstate)
          ((erp open-span parstate) (read-punctuator "(" parstate))
          ((erp exprs & parstate) (parse-argument-expressions parstate))
          ((erp close-span parstate) (read-punctuator ")" parstate)))
@@ -10791,7 +11343,10 @@
   ;;;;;;;;;;;;;;;;;;;;;;;;;;;;;;;;;;;;;;;;
 
   (define parse-attribute ((parstate parstatep))
-    :returns (mv erp (attr attribp) (span spanp) (new-parstate parstatep))
+    :returns (mv erp
+                 (attr attribp)
+                 (span spanp)
+                 (new-parstate parstatep :hyp (parstatep parstate)))
     :parents (parser parse-exprs/decls)
     :short "Parse an attribute."
     :long
@@ -10799,7 +11354,7 @@
      (xdoc::p
       "This is only used if GCC extensions are supported.
        See the ABNF grammar rule for @('attribute')."))
-    (b* (((reterr) (irr-attrib) (irr-span) (irr-parstate))
+    (b* (((reterr) (irr-attrib) (irr-span) parstate)
          ((erp ident ident-span parstate) (read-identifier parstate)) ; ident
          ((erp token & parstate) (read-token parstate)))
       (cond
@@ -10820,7 +11375,10 @@
   ;;;;;;;;;;;;;;;;;;;;;;;;;;;;;;;;;;;;;;;;
 
   (define parse-attribute-list ((parstate parstatep))
-    :returns (mv erp (attrs attrib-listp) (span spanp) (new-parstate parstatep))
+    :returns (mv erp
+                 (attrs attrib-listp)
+                 (span spanp)
+                 (new-parstate parstatep :hyp (parstatep parstate)))
     :parents (parser parse-exprs/decls)
     :short "Parse a list of one or more attributes, separated by commas."
     :long
@@ -10828,7 +11386,7 @@
      (xdoc::p
       "This is only used if GCC extensions are supported.
        See the ABNF grammar rule for @('attribute-list')."))
-    (b* (((reterr) nil (irr-span) (irr-parstate))
+    (b* (((reterr) nil (irr-span) parstate)
          (psize (parsize parstate))
          ((erp attr span parstate) (parse-attribute parstate)) ; attr
          ((unless (mbt (<= (parsize parstate) (1- psize))))
@@ -10855,7 +11413,7 @@
     :returns (mv erp
                  (attrspec attrib-specp)
                  (span spanp)
-                 (new-parstate parstatep))
+                 (new-parstate parstatep :hyp (parstatep parstate)))
     :parents (parser parse-exprs/decls)
     :short "Parse an attribute specifier."
     :long
@@ -10866,7 +11424,7 @@
      (xdoc::p
       "This is called after parsing the initial @('__attribute__'),
        whose span we pass to this parsing function as input."))
-    (b* (((reterr) (irr-attrib-spec) (irr-span) (irr-parstate))
+    (b* (((reterr) (irr-attrib-spec) (irr-span) parstate)
          ;; __attribute__
          ((erp & parstate) (read-punctuator "(" parstate)) ; __attribute__ (
          ((erp & parstate) (read-punctuator "(" parstate)) ; __attribute__ ( (
@@ -10885,7 +11443,7 @@
     :returns (mv erp
                  (attrspecs attrib-spec-listp)
                  (span spanp)
-                 (new-parstate parstatep))
+                 (new-parstate parstatep :hyp (parstatep parstate)))
     :parents (parser parse-exprs/decls)
     :short "Parse zero or more attribute specifiers."
     :long
@@ -10912,7 +11470,7 @@
        this parsing function always returns the empty list,
        because @('__attribute__') is a keyword
        only if GCC extensions are supported."))
-    (b* (((reterr) nil (irr-span) (irr-parstate))
+    (b* (((reterr) nil (irr-span) parstate)
          ((erp token first-span parstate) (read-token parstate))
          ((unless (token-keywordp token "__attribute__"))
           (b* ((parstate (if token (unread-token parstate) parstate)))
@@ -11821,7 +12379,7 @@
   :returns (mv erp
                (asmspec asm-name-specp)
                (span spanp)
-               (new-parstate parstatep))
+               (new-parstate parstatep :hyp (parstatep parstate)))
   :short "Parse an assembler name specifier."
   :long
   (xdoc::topstring
@@ -11836,7 +12394,7 @@
      and return its abstract syntax representation.
      We ensure that there is at least one string literal;
      see grammar rule for @('asm-name-specifier'), which uses @('1*')."))
-  (b* (((reterr) (irr-asm-name-spec) (irr-span) (irr-parstate))
+  (b* (((reterr) (irr-asm-name-spec) (irr-span) parstate)
        ;; asm-or-__asm__
        ((erp & parstate) (read-punctuator "(" parstate)) ; asm-or-__asm__ (
        ((erp token span parstate) (read-token parstate))
@@ -11873,7 +12431,7 @@
   :returns (mv erp
                (asmspec? asm-name-spec-optionp)
                (span spanp)
-               (new-parstate parstatep))
+               (new-parstate parstatep :hyp (parstatep parstate)))
   :short "Parse an optional assembler name specifier."
   :long
   (xdoc::topstring
@@ -11885,7 +12443,7 @@
      Otherwise, we put back the token
      and return no assembler name specifier;
      in this case, the returned span is an irrelevant one."))
-  (b* (((reterr) nil (irr-span) (irr-parstate))
+  (b* (((reterr) nil (irr-span) parstate)
        ((erp token span parstate) (read-token parstate)))
     (cond
      ((token-keywordp token "asm")
@@ -11909,14 +12467,14 @@
   :returns (mv erp
                (initdeclor initdeclorp)
                (span spanp)
-               (new-parstate parstatep))
+               (new-parstate parstatep :hyp (parstatep parstate)))
   :short "Parse an initializer declarator."
   :long
   (xdoc::topstring
    (xdoc::p
     "An initializer declarator consists of a declarator,
      optionally followed by an equal sign and an initializer."))
-  (b* (((reterr) (irr-initdeclor) (irr-span) (irr-parstate))
+  (b* (((reterr) (irr-initdeclor) (irr-span) parstate)
        ((erp declor span parstate) (parse-declarator parstate)) ; declor
        ((erp token & parstate) (read-token parstate)))
     (cond
@@ -11953,7 +12511,7 @@
   :returns (mv erp
                (initdeclors initdeclor-listp)
                (span spanp)
-               (new-parstate parstatep))
+               (new-parstate parstatep :hyp (parstatep parstate)))
   :short "Parse a list of one or more initializer declarators."
   :long
   (xdoc::topstring
@@ -11961,7 +12519,7 @@
     "We parse the first one, which must be present.
      If there is a comma after that,
      we recursively parse one or more after the comma."))
-  (b* (((reterr) nil (irr-span) (irr-parstate))
+  (b* (((reterr) nil (irr-span) parstate)
        ((erp initdeclor span parstate) ; initdeclor
         (parse-init-declarator parstate))
        ((erp token & parstate) (read-token parstate)))
@@ -12001,7 +12559,10 @@
 ;;;;;;;;;;;;;;;;;;;;;;;;;;;;;;;;;;;;;;;;;;;;;;;;;;;;;;;;;;;;;;;;;;;;;;;;;;;;;;;;
 
 (define parse-declaration ((parstate parstatep))
-  :returns (mv erp (decl declp) (span spanp) (new-parstate parstatep))
+  :returns (mv erp
+               (decl declp)
+               (span spanp)
+               (new-parstate parstatep :hyp (parstatep parstate)))
   :short "Parse a declaration."
   :long
   (xdoc::topstring
@@ -12019,7 +12580,7 @@
      and we must also allow for an @('__extension__') keyword
      just before the declaration.
      See the ABNF grammar rule for @('declaration')."))
-  (b* (((reterr) (irr-decl) (irr-span) (irr-parstate))
+  (b* (((reterr) (irr-decl) (irr-span) parstate)
        ((erp token span parstate) (read-token parstate)))
     (cond
      ;; If token may start a declaration specifier, we put it back and
@@ -12035,7 +12596,8 @@
             (if (and (token-keywordp token "__extension__")
                      (parstate->gcc parstate))
                 (mv t parstate)
-              (mv nil (unread-token parstate))))
+              (b* ((parstate (unread-token parstate)))
+                (mv nil parstate))))
            ;; [__extension__]
            ((erp declspecs span parstate) ; [__extension__] declspecs
             (parse-declaration-specifiers nil parstate))
@@ -12173,7 +12735,10 @@
 ;;;;;;;;;;;;;;;;;;;;;;;;;;;;;;;;;;;;;;;;;;;;;;;;;;;;;;;;;;;;;;;;;;;;;;;;;;;;;;;;
 
 (define parse-declaration-list ((parstate parstatep))
-  :returns (mv erp (decls decl-listp) (span spanp) (new-parstate parstatep))
+  :returns (mv erp
+               (decls decl-listp)
+               (span spanp)
+               (new-parstate parstatep :hyp (parstatep parstate)))
   :short "Parse a list of one or more declarations."
   :long
   (xdoc::topstring
@@ -12183,7 +12748,7 @@
      because the only place where we parse declaration lists
      is in function definitions, between declarator and body.
      Otherwise we recursively call this function to parse more."))
-  (b* (((reterr) nil (irr-span) (irr-parstate))
+  (b* (((reterr) nil (irr-span) parstate)
        ((erp decl span parstate) (parse-declaration parstate)) ; decl
        ((erp token & parstate) (read-token parstate)))
     (cond
@@ -12223,7 +12788,7 @@
   :returns (mv erp
                (decl/stmt amb?-decl/stmt-p)
                (span spanp)
-               (new-parstate parstatep))
+               (new-parstate parstatep :hyp (parstatep parstate)))
   :short "Parse a declaration or a statement."
   :long
   (xdoc::topstring
@@ -12245,7 +12810,7 @@
      If both succeed, there is an ambiguity,
      which we return as such.
      If none succeeds, it is an error."))
-  (b* (((reterr) (irr-amb?-decl/stmt) (irr-span) (irr-parstate))
+  (b* (((reterr) (irr-amb?-decl/stmt) (irr-span) parstate)
        (parstate (record-checkpoint parstate)) ; we will backtrack here
        (psize (parsize parstate))
        ((mv erp expr span-expr parstate) (parse-expression parstate)))
@@ -12263,7 +12828,7 @@
               ;; no larger than the initial one,
               ;; so we just return the empty parser state.
               ;; This is just logical: execution stops at the RAISE above.
-              (b* ((parstate (init-parstate nil nil)))
+              (b* ((parstate (init-parstate nil nil parstate)))
                 (reterr t)))
              ((erp decl span parstate) (parse-declaration parstate)))
           (retok (amb?-decl/stmt-decl decl) span parstate))
@@ -12291,7 +12856,7 @@
                   ;; so we just return the empty parser state.
                   ;; This is just logical:
                   ;; execution stops at the RAISE above.
-                  (b* ((parstate (init-parstate nil nil)))
+                  (b* ((parstate (init-parstate nil nil parstate)))
                     (reterr t)))
                  (parstate
                   (record-checkpoint parstate)) ; we may backtrack again
@@ -12314,7 +12879,7 @@
                         ;; so we just return the empty parser state.
                         ;; This is just logical:
                         ;; execution stops at the RAISE above.
-                        (b* ((parstate (init-parstate nil nil)))
+                        (b* ((parstate (init-parstate nil nil parstate)))
                           (reterr t)))
                        ((mv erp expr1 span-expr1 parstate)
                         (parse-expression parstate))
@@ -12388,7 +12953,7 @@
                 ;; so we just return the empty parser state.
                 ;; This is just logical:
                 ;; execution stops at the RAISE above.
-                (b* ((parstate (init-parstate nil nil)))
+                (b* ((parstate (init-parstate nil nil parstate)))
                   (reterr t)))
                ((erp decl span parstate) (parse-declaration parstate)))
             (retok (amb?-decl/stmt-decl decl) span parstate))))))
@@ -12421,7 +12986,10 @@
   ;;;;;;;;;;;;;;;;;;;;;;;;;;;;;;;;;;;;;;;;
 
   (define parse-statement ((parstate parstatep))
-    :returns (mv erp (stmt stmtp) (span spanp) (new-parstate parstatep))
+    :returns (mv erp
+                 (stmt stmtp)
+                 (span spanp)
+                 (new-parstate parstatep :hyp (parstatep parstate)))
     :parents (parser parse-stmts/blocks)
     :short "Parse a statement."
     :long
@@ -12452,7 +13020,7 @@
        In other words, we may fail to accept the case of
        a declaration that starts with a @('typedef') name for now.
        We plan to rectify this situation soon."))
-    (b* (((reterr) (irr-stmt) (irr-span) (irr-parstate))
+    (b* (((reterr) (irr-stmt) (irr-span) parstate)
          ((erp token span parstate) (read-token parstate)))
       (cond
        ;; If token is an identifier,
@@ -13094,7 +13662,10 @@
   ;;;;;;;;;;;;;;;;;;;;;;;;;;;;;;;;;;;;;;;;
 
   (define parse-block-item ((parstate parstatep))
-    :returns (mv erp (item block-itemp) (span spanp) (new-parstate parstatep))
+    :returns (mv erp
+                 (item block-itemp)
+                 (span spanp)
+                 (new-parstate parstatep :hyp (parstatep parstate)))
     :parents (parser parse-stmts/blocks)
     :short "Parse a block item."
     :long
@@ -13107,7 +13678,7 @@
        the overlap cannot be disambiguated purely syntactically.
        Thus, under the appropriate conditions,
        we parse a possibly ambiguous declaration or statement."))
-    (b* (((reterr) (irr-block-item) (irr-span) (irr-parstate))
+    (b* (((reterr) (irr-block-item) (irr-span) parstate)
          ((erp token & parstate) (read-token parstate)))
       (cond
        ;; If token is an identifier, we need to read another token.
@@ -13170,7 +13741,7 @@
     :returns (mv erp
                  (items block-item-listp)
                  (span spanp)
-                 (new-parstate parstatep))
+                 (new-parstate parstatep :hyp (parstatep parstate)))
     :parents (parser parse-stmts/blocks)
     :short "Parse a list of one or more block items."
     :long
@@ -13179,7 +13750,7 @@
       "We parse the first block item, which must be present.
        Then, unless we have a closed curly brace,
        we recursively parse one or more block items."))
-    (b* (((reterr) nil (irr-span) (irr-parstate))
+    (b* (((reterr) nil (irr-span) parstate)
          (psize (parsize parstate))
          ((erp item span parstate) (parse-block-item parstate)) ; item
          ((unless (mbt (<= (parsize parstate) (1- psize))))
@@ -13269,7 +13840,10 @@
 ;;;;;;;;;;;;;;;;;;;;;;;;;;;;;;;;;;;;;;;;;;;;;;;;;;;;;;;;;;;;;;;;;;;;;;;;;;;;;;;;
 
 (define parse-external-declaration ((parstate parstatep))
-  :returns (mv erp (extdecl extdeclp) (span spanp) (new-parstate parstatep))
+  :returns (mv erp
+               (extdecl extdeclp)
+               (span spanp)
+               (new-parstate parstatep :hyp (parstatep parstate)))
   :short "Parse an external declaration."
   :long
   (xdoc::topstring
@@ -13295,7 +13869,7 @@
     "If GCC extensions are supported, we must also taken into account
      the possible presence of attributes and assembler name specifiers,
      as well as of an @('__external__') keyword."))
-  (b* (((reterr) (irr-extdecl) (irr-span) (irr-parstate))
+  (b* (((reterr) (irr-extdecl) (irr-span) parstate)
        ((erp token span parstate) (read-token parstate)))
     (cond
      ;; If token is the keyword '_Static_assert',
@@ -13312,7 +13886,8 @@
             (if (and (token-keywordp token "__extension__")
                      (parstate->gcc parstate))
                 (mv t parstate)
-              (mv nil (if token (unread-token parstate) parstate))))
+              (b* ((parstate (if token (unread-token parstate) parstate)))
+                (mv nil parstate))))
            ;; [__extension__]
            ((erp declspecs span parstate) ; [__extension__] declspecs
             (parse-declaration-specifiers nil parstate))
@@ -13705,7 +14280,7 @@
                (extdecls extdecl-listp)
                (span spanp)
                (eof-pos positionp)
-               (new-parstate parstatep))
+               (new-parstate parstatep :hyp (parstatep parstate)))
   :short "Parse a list of one or more external declarations."
   :long
   (xdoc::topstring
@@ -13720,7 +14295,7 @@
     "We parse the first external declaration, which must be present.
      Then, unless we have reached the end of the file,
      we recursively parse more external declarations."))
-  (b* (((reterr) nil (irr-span) (irr-position) (irr-parstate))
+  (b* (((reterr) nil (irr-span) (irr-position) parstate)
        ((erp extdecl first-span parstate) ; extdecl
         (parse-external-declaration parstate))
        ((erp token span parstate) (read-token parstate))
@@ -13756,7 +14331,9 @@
 ;;;;;;;;;;;;;;;;;;;;;;;;;;;;;;;;;;;;;;;;;;;;;;;;;;;;;;;;;;;;;;;;;;;;;;;;;;;;;;;;
 
 (define parse-translation-unit ((parstate parstatep))
-  :returns (mv erp (tunit transunitp) (new-parstate parstatep))
+  :returns (mv erp
+               (tunit transunitp)
+               (new-parstate parstatep :hyp (parstatep parstate)))
   :short "Parse a translation unit."
   :long
   (xdoc::topstring
@@ -13775,7 +14352,7 @@
      this means that, since the file is not empty,
      the last character is a new-line,
      otherwise that position would be at a non-zero column."))
-  (b* (((reterr) (irr-transunit) (irr-parstate))
+  (b* (((reterr) (irr-transunit) parstate)
        ((erp extdecls & eof-pos parstate)
         (parse-external-declaration-list parstate))
        ((unless (= (position->column eof-pos) 0))
@@ -13806,24 +14383,33 @@
     "We also pass a flag saying whether GCC extensions should be accepted.")
    (xdoc::p
     "If successful, the result is a translation unit.
-     We initialize the parser state with the data bytes,
+     We create a local stobj with the parser state,
+     we initialize it with the data bytes,
      and we attempt to parse them as a translation unit.
-     The final parser state is discarded, since it is no longer needed.")
+     The final parser state is discarded, as is the case for local stobjs,
+     since it is no longer needed.")
    (xdoc::p
     "If an error occurs, we enhance it with
      information about the file path.
      It is the case that @('erp') is a message,
      but currently we do not have that information statically available,
      so we add a run-time check that should always succeed."))
-  (b* (((reterr) (irr-transunit))
-       (parstate (init-parstate data gcc))
-       ((mv erp tunit &) (parse-translation-unit parstate))
-       ((when erp)
-        (b* (((unless (msgp erp))
-              (raise "Internal error: ~x0 is not a message." erp)
-              (reterr t)))
-          (reterr (msg "Error in file ~x0: ~@1" (filepath->unwrap path) erp)))))
-    (retok tunit)))
+  (with-local-stobj
+    parstate
+    (mv-let (erp tunit parstate)
+        (b* ((parstate (init-parstate data gcc parstate))
+             ((mv erp tunit parstate) (parse-translation-unit parstate)))
+          (if erp
+              (if (msgp erp)
+                  (mv (msg "Error in file ~x0: ~@1"
+                           (filepath->unwrap path) erp)
+                      (irr-transunit)
+                      parstate)
+                (prog2$
+                 (raise "Internal error: ~x0 is not a message." erp)
+                 (mv t (irr-transunit) parstate)))
+            (mv nil tunit parstate)))
+      (mv erp tunit))))
 
 ;;;;;;;;;;;;;;;;;;;;;;;;;;;;;;;;;;;;;;;;;;;;;;;;;;;;;;;;;;;;;;;;;;;;;;;;;;;;;;;;
 
