books/kestrel/c/syntax/tests/parser.lisp
@@ -12,6 +12,8 @@
 
 (include-book "../parser")
 
+(include-book "std/testing/assert-bang-stobj" :dir :system)
+
 ;;;;;;;;;;;;;;;;;;;;;;;;;;;;;;;;;;;;;;;;;;;;;;;;;;;;;;;;;;;;;;;;;;;;;;;;;;;;;;;;
 
 ; Test messages.
@@ -154,18 +156,20 @@
 ;;;;;;;;;;;;;;;;;;;;;;;;;;;;;;;;;;;;;;;;
 
 (defmacro test-init-parstate (list gcc)
-  `(assert-event
-    (equal (init-parstate ,list ,gcc)
-           (parstate ,list
-                     (position-init)
-                     nil
-                     nil
-                     nil
-                     0
-                     nil
-                     nil
-                     ,gcc
-                     (len ,list)))))
+  `(assert!-stobj
+    (b* ((parstate (init-parstate ,list ,gcc parstate)))
+      (mv (and (equal (parstate->bytes parstate) ,list)
+               (equal (parstate->position parstate) (position-init))
+               (equal (parstate->chars-read parstate) nil)
+               (equal (parstate->chars-unread parstate) nil)
+               (equal (parstate->tokens-read parstate) nil)
+               (equal (parstate->tokens-read-len parstate) 0)
+               (equal (parstate->tokens-unread parstate) nil)
+               (equal (parstate->checkpoints parstate) nil)
+               (equal (parstate->gcc parstate) ,gcc)
+               (equal (parstate->size parstate) (len ,list)))
+          parstate))
+    parstate))
 
 (test-init-parstate nil nil)
 
@@ -185,17 +189,29 @@
 
 ;;;;;;;;;;;;;;;;;;;;;;;;;;;;;;;;;;;;;;;;
 
-(assert-event
- (equal (parsize (init-parstate nil nil)) 0))
+(assert!-stobj
+ (b* ((parstate (init-parstate nil nil parstate)))
+   (mv (equal (parsize parstate) 0)
+       parstate))
+ parstate)
 
-(assert-event
- (equal (parsize (init-parstate nil t)) 0))
+(assert!-stobj
+ (b* ((parstate (init-parstate nil t parstate)))
+   (mv (equal (parsize parstate) 0)
+       parstate))
+ parstate)
 
-(assert-event
- (equal (parsize (init-parstate (list 72 99 21) nil)) 3))
+(assert!-stobj
+ (b* ((parstate (init-parstate (list 72 99 21) nil parstate)))
+   (mv (equal (parsize parstate) 3)
+       parstate))
+ parstate)
 
-(assert-event
- (equal (parsize (init-parstate (list 72 99 21) t)) 3))
+(assert!-stobj
+ (b* ((parstate (init-parstate (list 72 99 21) t parstate)))
+   (mv (equal (parsize parstate) 3)
+       parstate))
+ parstate)
 
 ;;;;;;;;;;;;;;;;;;;;;;;;;;;;;;;;;;;;;;;;;;;;;;;;;;;;;;;;;;;;;;;;;;;;;;;;;;;;;;;;
 
@@ -203,312 +219,372 @@
 
 ;;;;;;;;;;;;;;;;;;;;;;;;;;;;;;;;;;;;;;;;
 
-(assert-event ; empty file
- (b* ((pstate0 (init-parstate nil nil))
-      ((mv erp char? pos pstate) (read-char pstate0)))
-   (and (not erp)
-        (not char?)
-        (equal pos (position 1 0)) ; just past end of (empty) file
-        (equal pstate pstate0))))
+(assert!-stobj ; empty file
+ (b* ((parstate (init-parstate nil nil parstate))
+      (pstate0 (to-parstate$ parstate))
+      ((mv erp char? pos parstate) (read-char parstate)))
+   (mv (and (not erp)
+            (not char?)
+            (equal pos (position 1 0)) ; just past end of (empty) file
+            (equal (to-parstate$ parstate)
+                   pstate0))
+       parstate))
+ parstate)
 
-(assert-event ; disallowed character 0
- (b* (((mv erp & & &) (read-char (init-parstate (list 0) nil)))
+(assert!-stobj ; disallowed character 0
+ (b* ((parstate (init-parstate (list 0) nil parstate))
+      ((mv erp & & parstate) (read-char parstate))
       (- (cw "~@0" erp)))
-   erp))
+   (mv erp parstate))
+ parstate)
 
-(assert-event ; character 32
- (b* ((pstate0 (init-parstate (list 32 1 2 3) nil))
-      ((mv erp char? pos pstate) (read-char pstate0)))
-   (and (not erp)
-        (equal char? 32)
-        (equal pos (position 1 0))
-        (equal pstate
-               (change-parstate
-                pstate0
-                :bytes (list 1 2 3)
-                :position (position 1 1)
-                :chars-read (list (char+position 32 (position 1 0)))
-                :size 3)))))
+(assert!-stobj ; character 32
+ (b* ((parstate (init-parstate (list 32 1 2 3) nil parstate))
+      (pstate0 (to-parstate$ parstate))
+      ((mv erp char? pos parstate) (read-char parstate)))
+   (mv (and (not erp)
+            (equal char? 32)
+            (equal pos (position 1 0))
+            (equal (to-parstate$ parstate)
+                   (change-parstate$
+                    pstate0
+                    :bytes (list 1 2 3)
+                    :position (position 1 1)
+                    :chars-read (list (char+position 32 (position 1 0)))
+                    :size 3)))
+       parstate))
+ parstate)
 
-(assert-event ; line feed
- (b* ((pstate0 (init-parstate (list 10 1 2 3) nil))
-      ((mv erp char? pos pstate) (read-char pstate0)))
-   (and (not erp)
-        (equal char? 10)
-        (equal pos (position 1 0))
-        (equal pstate
-               (change-parstate
-                pstate0
-                :bytes (list 1 2 3)
-                :position (position 2 0)
-                :chars-read (list (char+position 10 (position 1 0)))
-                :size 3)))))
+(assert!-stobj ; line feed
+ (b* ((parstate (init-parstate (list 10 1 2 3) nil parstate))
+      (pstate0 (to-parstate$ parstate))
+      ((mv erp char? pos parstate) (read-char parstate)))
+   (mv (and (not erp)
+            (equal char? 10)
+            (equal pos (position 1 0))
+            (equal (to-parstate$ parstate)
+                   (change-parstate$
+                    pstate0
+                    :bytes (list 1 2 3)
+                    :position (position 2 0)
+                    :chars-read (list (char+position 10 (position 1 0)))
+                    :size 3)))
+       parstate))
+ parstate)
 
-(assert-event ; carriage return
- (b* ((pstate0 (init-parstate (list 13 1 2 3) nil))
-      ((mv erp char? pos pstate) (read-char pstate0)))
-   (and (not erp)
-        (equal char? 10)
-        (equal pos (position 1 0))
-        (equal pstate
-               (change-parstate
-                pstate0
-                :bytes (list 1 2 3)
-                :position (position 2 0)
-                :chars-read (list (char+position 10 (position 1 0)))
-                :size 3)))))
+(assert!-stobj ; carriage return
+ (b* ((parstate (init-parstate (list 13 1 2 3) nil parstate))
+      (pstate0 (to-parstate$ parstate))
+      ((mv erp char? pos parstate) (read-char parstate)))
+   (mv (and (not erp)
+            (equal char? 10)
+            (equal pos (position 1 0))
+            (equal (to-parstate$ parstate)
+                   (change-parstate$
+                    pstate0
+                    :bytes (list 1 2 3)
+                    :position (position 2 0)
+                    :chars-read (list (char+position 10 (position 1 0)))
+                    :size 3)))
+       parstate))
+ parstate)
 
-(assert-event ; carriage return + line feed
- (b* ((pstate0 (init-parstate (list 13 10 1 2 3) nil))
-      ((mv erp char? pos pstate) (read-char pstate0)))
-   (and (not erp)
-        (equal char? 10)
-        (equal pos (position 1 0))
-        (equal pstate
-               (change-parstate
-                pstate0
-                :bytes (list 1 2 3)
-                :position (position 2 0)
-                :chars-read (list (char+position 10 (position 1 0)))
-                :size 3)))))
+(assert!-stobj ; carriage return + line feed
+ (b* ((parstate (init-parstate (list 13 10 1 2 3) nil parstate))
+      (pstate0 (to-parstate$ parstate))
+      ((mv erp char? pos parstate) (read-char parstate)))
+   (mv (and (not erp)
+            (equal char? 10)
+            (equal pos (position 1 0))
+            (equal (to-parstate$ parstate)
+                   (change-parstate$
+                    pstate0
+                    :bytes (list 1 2 3)
+                    :position (position 2 0)
+                    :chars-read (list (char+position 10 (position 1 0)))
+                    :size 3)))
+       parstate))
+ parstate)
 
-(assert-event ; disallowed byte 255
- (b* ((pstate0 (init-parstate (list 255) nil))
-      ((mv erp & & &) (read-char pstate0))
+(assert!-stobj ; disallowed byte 255
+ (b* ((parstate (init-parstate (list 255) nil parstate))
+      ((mv erp & & parstate) (read-char parstate))
       (- (cw "~@0" erp)))
-   erp))
+   (mv erp parstate))
+ parstate)
 
-(assert-event ; 2-byte UTF-8 encoding of Greek capital letter sigma
- (b* ((pstate0 (init-parstate (acl2::string=>nats "Σ") nil))
-      ((mv erp char? pos pstate) (read-char pstate0)))
-   (and (not erp)
-        (equal char? #x03a3)
-        (equal pos (position 1 0))
-        (equal pstate
-               (change-parstate
-                pstate0
-                :bytes nil
-                :position (position 1 1)
-                :chars-read (list (char+position #x03a3 (position 1 0)))
-                :size 0)))))
+(assert!-stobj ; 2-byte UTF-8 encoding of Greek capital letter sigma
+ (b* ((parstate (init-parstate (acl2::string=>nats "Σ") nil parstate))
+      (pstate0 (to-parstate$ parstate))
+      ((mv erp char? pos parstate) (read-char parstate)))
+   (mv (and (not erp)
+            (equal char? #x03a3)
+            (equal pos (position 1 0))
+            (equal (to-parstate$ parstate)
+                   (change-parstate$
+                    pstate0
+                    :bytes nil
+                    :position (position 1 1)
+                    :chars-read (list (char+position #x03a3 (position 1 0)))
+                    :size 0)))
+       parstate))
+ parstate)
 
-(assert-event ; invalid 2-byte UTF-8 encoding of 0
- (b* ((pstate0 (init-parstate (list #b11000000 #b10000000) nil))
-      ((mv erp & & &) (read-char pstate0))
+(assert!-stobj ; invalid 2-byte UTF-8 encoding of 0
+ (b* ((parstate (init-parstate (list #b11000000 #b10000000) nil parstate))
+      ((mv erp & & parstate) (read-char parstate))
       (- (cw "~@0" erp)))
-   erp))
+   (mv erp parstate))
+ parstate)
 
-(assert-event ; 3-byte UTF-8 encoding of anticlockwise top semicircle arrow
- (b* ((pstate0 (init-parstate (acl2::string=>nats "↺") nil))
-      ((mv erp char? pos pstate) (read-char pstate0)))
-   (and (not erp)
-        (equal char? #x21ba)
-        (equal pos (position 1 0))
-        (equal pstate
-               (change-parstate
-                pstate0
-                :bytes nil
-                :position (position 1 1)
-                :chars-read (list (char+position #x21ba (position 1 0)))
-                :size 0)))))
+(assert!-stobj ; 3-byte UTF-8 encoding of anticlockwise top semicircle arrow
+ (b* ((parstate (init-parstate (acl2::string=>nats "↺") nil parstate))
+      (pstate0 (to-parstate$ parstate))
+      ((mv erp char? pos parstate) (read-char parstate)))
+   (mv (and (not erp)
+            (equal char? #x21ba)
+            (equal pos (position 1 0))
+            (equal (to-parstate$ parstate)
+                   (change-parstate$
+                    pstate0
+                    :bytes nil
+                    :position (position 1 1)
+                    :chars-read (list (char+position #x21ba (position 1 0)))
+                    :size 0)))
+       parstate))
+ parstate)
 
-(assert-event ; disallowed 3-byte UTF-8 encoding
- (b* ((pstate0
-       (init-parstate (list #b11100010 #b10000000 #b10101010) nil)) ; 202Ah
-      ((mv erp & & &) (read-char pstate0))
+(assert!-stobj ; disallowed 3-byte UTF-8 encoding
+ (b* ((parstate (init-parstate (list #b11100010 #b10000000 #b10101010) ; 202Ah
+                               nil
+                               parstate))
+      ((mv erp & & parstate) (read-char parstate))
       (- (cw "~@0" erp)))
-   erp))
+   (mv erp parstate))
+ parstate)
 
-(assert-event ; invalid 3-byte UTF-8 encoding of 0
- (b* ((pstate0 (init-parstate (list #b11100000 #b10000000 #b10000000) nil))
-      ((mv erp & & &) (read-char pstate0))
+(assert!-stobj ; invalid 3-byte UTF-8 encoding of 0
+ (b* ((parstate (init-parstate (list #b11100000 #b10000000 #b10000000)
+                               nil
+                               parstate))
+      ((mv erp & & parstate) (read-char parstate))
       (- (cw "~@0" erp)))
-   erp))
+   (mv erp parstate))
+ parstate)
 
-(assert-event ; 4-byte UTF-8 encoding of musical symbol eighth note
- (b* ((pstate0 (init-parstate (acl2::string=>nats "𝅘𝅥𝅮") nil))
-      ((mv erp char? pos pstate) (read-char pstate0)))
-   (and (not erp)
-        (equal char? #x1d160)
-        (equal pos (position 1 0))
-        (equal pstate
-               (change-parstate
-                pstate0
-                :bytes nil
-                :position (position 1 1)
-                :chars-read (list (char+position #x1d160 (position 1 0)))
-                :size 0)))))
+(assert!-stobj ; 4-byte UTF-8 encoding of musical symbol eighth note
+ (b* ((parstate (init-parstate (acl2::string=>nats "𝅘𝅥𝅮") nil parstate))
+      (pstate0 (to-parstate$ parstate))
+      ((mv erp char? pos parstate) (read-char parstate)))
+   (mv (and (not erp)
+            (equal char? #x1d160)
+            (equal pos (position 1 0))
+            (equal (to-parstate$ parstate)
+                   (change-parstate$
+                    pstate0
+                    :bytes nil
+                    :position (position 1 1)
+                    :chars-read (list (char+position #x1d160 (position 1 0)))
+                    :size 0)))
+       parstate))
+ parstate)
 
-(assert-event ; invalid 4-byte UTF-8 encoding of 0
- (b* ((pstate0
-       (init-parstate (list #b11110000 #b10000000 #b10000000 #b10000000) nil))
-      ((mv erp & & &) (read-char pstate0))
+(assert!-stobj ; invalid 4-byte UTF-8 encoding of 0
+ (b* ((parstate (init-parstate (list #b11110000 #b10000000 #b10000000 #b10000000)
+                               nil
+                               parstate))
+      ((mv erp & & parstate) (read-char parstate))
       (- (cw "~@0" erp)))
-   erp))
+   (mv erp parstate))
+ parstate)
 
-(assert-event ; invalid 4-byte UTF-8 encoding of 1FFFFFh
- (b* ((pstate0
-       (init-parstate (list #b11110111 #b10111111 #b10111111 #b10111111) nil))
-      ((mv erp & & &) (read-char pstate0))
+(assert!-stobj ; invalid 4-byte UTF-8 encoding of 1FFFFFh
+ (b* ((parstate (init-parstate
+                 (list #b11110111 #b10111111 #b10111111 #b10111111)
+                 nil
+                 parstate))
+      ((mv erp & & parstate) (read-char parstate))
       (- (cw "~@0" erp)))
-   erp))
+   (mv erp parstate))
+ parstate)
 
 ;;;;;;;;;;;;;;;;;;;;;;;;;;;;;;;;;;;;;;;;
 
-(assert-event
- (b* ((pstate0 (init-parstate (list 65 66 67) nil)) ; A B C
-      ((mv erp1 char-a pos-a pstate1) (read-char pstate0))
-      ((mv erp2 char-b pos-b pstate2) (read-char pstate1))
-      (pstate3 (unread-char pstate2))
-      ((mv erp4 char-b2 pos-b2 pstate4) (read-char pstate3))
-      ((mv erp5 char-c pos-c pstate5) (read-char pstate4))
-      ((mv erp6 char-eof pos-eof pstate6) (read-char pstate5)))
-   (and (not erp1)
-        (not erp2)
-        (not erp4)
-        (not erp5)
-        (not erp6)
-        (equal char-a 65)
-        (equal char-b 66)
-        (equal char-b2 66)
-        (equal char-c 67)
-        (equal char-eof nil)
-        (equal pos-a (position 1 0))
-        (equal pos-b (position 1 1))
-        (equal pos-b2 (position 1 1))
-        (equal pos-c (position 1 2))
-        (equal pos-eof (position 1 3))
-        (equal pstate1
-               (change-parstate
-                pstate0
-                :bytes (list 66 67)
-                :position (position 1 1)
-                :chars-read (list (char+position 65 (position 1 0)))
-                :size 2))
-        (equal pstate2
-               (change-parstate
-                pstate1
-                :bytes (list 67)
-                :position (position 1 2)
-                :chars-read (list (char+position 66 (position 1 1))
-                                  (char+position 65 (position 1 0)))
-                :size 1))
-        (equal pstate3
-               (change-parstate
-                pstate2
-                :chars-read (list (char+position 65 (position 1 0)))
-                :chars-unread (list (char+position 66 (position 1 1)))
-                :size 2))
-        (equal pstate4
-               (change-parstate
-                pstate3
-                :chars-read (list (char+position 66 (position 1 1))
-                                  (char+position 65 (position 1 0)))
-                :chars-unread nil
-                :size 1))
-        (equal pstate5
-               (change-parstate
-                pstate4
-                :bytes nil
-                :position (position 1 3)
-                :chars-read (list (char+position 67 (position 1 2))
-                                  (char+position 66 (position 1 1))
-                                  (char+position 65 (position 1 0)))
-                :size 0))
-        (equal pstate6
-               pstate5))))
+(assert!-stobj
+ (b* ((parstate (init-parstate (list 65 66 67) nil parstate)) ; A B C
+      (pstate0 (to-parstate$ parstate))
+      ((mv erp1 char-a pos-a parstate) (read-char parstate))
+      (pstate1 (to-parstate$ parstate))
+      ((mv erp2 char-b pos-b parstate) (read-char parstate))
+      (pstate2 (to-parstate$ parstate))
+      (parstate (unread-char parstate))
+      (pstate3 (to-parstate$ parstate))
+      ((mv erp4 char-b2 pos-b2 parstate) (read-char parstate))
+      (pstate4 (to-parstate$ parstate))
+      ((mv erp5 char-c pos-c parstate) (read-char parstate))
+      (pstate5 (to-parstate$ parstate))
+      ((mv erp6 char-eof pos-eof parstate) (read-char parstate))
+      (pstate6 (to-parstate$ parstate)))
+   (mv (and (not erp1)
+            (not erp2)
+            (not erp4)
+            (not erp5)
+            (not erp6)
+            (equal char-a 65)
+            (equal char-b 66)
+            (equal char-b2 66)
+            (equal char-c 67)
+            (equal char-eof nil)
+            (equal pos-a (position 1 0))
+            (equal pos-b (position 1 1))
+            (equal pos-b2 (position 1 1))
+            (equal pos-c (position 1 2))
+            (equal pos-eof (position 1 3))
+            (equal pstate1
+                   (change-parstate$
+                    pstate0
+                    :bytes (list 66 67)
+                    :position (position 1 1)
+                    :chars-read (list (char+position 65 (position 1 0)))
+                    :size 2))
+            (equal pstate2
+                   (change-parstate$
+                    pstate1
+                    :bytes (list 67)
+                    :position (position 1 2)
+                    :chars-read (list (char+position 66 (position 1 1))
+                                      (char+position 65 (position 1 0)))
+                    :size 1))
+            (equal pstate3
+                   (change-parstate$
+                    pstate2
+                    :chars-read (list (char+position 65 (position 1 0)))
+                    :chars-unread (list (char+position 66 (position 1 1)))
+                    :size 2))
+            (equal pstate4
+                   (change-parstate$
+                    pstate3
+                    :chars-read (list (char+position 66 (position 1 1))
+                                      (char+position 65 (position 1 0)))
+                    :chars-unread nil
+                    :size 1))
+            (equal pstate5
+                   (change-parstate$
+                    pstate4
+                    :bytes nil
+                    :position (position 1 3)
+                    :chars-read (list (char+position 67 (position 1 2))
+                                      (char+position 66 (position 1 1))
+                                      (char+position 65 (position 1 0)))
+                    :size 0))
+            (equal pstate6
+                   pstate5))
+       parstate))
+ parstate)
 
-(assert-event
- (b* ((pstate0 (init-parstate (list 65 10 66) nil)) ; A LF B
-      ((mv erp1 char-a pos-a pstate1) (read-char pstate0))
-      ((mv erp2 char-nl pos-nl pstate2) (read-char pstate1))
-      (pstate3 (unread-chars 2 pstate2))
-      ((mv erp4 char-a2 pos-a2 pstate4) (read-char pstate3))
-      ((mv erp5 char-nl2 pos-nl2 pstate5) (read-char pstate4))
-      (pstate6 (unread-char pstate5))
-      ((mv erp7 char-nl3 pos-nl3 pstate7) (read-char pstate6))
-      ((mv erp8 char-b pos-b pstate8) (read-char pstate7))
-      ((mv erp9 char-eof pos-eof pstate9) (read-char pstate8)))
-   (and (not erp1)
-        (not erp2)
-        (not erp4)
-        (not erp5)
-        (not erp7)
-        (not erp8)
-        (not erp9)
-        (equal char-a 65)
-        (equal char-nl 10)
-        (equal char-a2 65)
-        (equal char-nl2 10)
-        (equal char-nl3 10)
-        (equal char-b 66)
-        (equal char-eof nil)
-        (equal pos-a (position 1 0))
-        (equal pos-a2 (position 1 0))
-        (equal pos-nl (position 1 1))
-        (equal pos-nl2 (position 1 1))
-        (equal pos-nl3 (position 1 1))
-        (equal pos-b (position 2 0))
-        (equal pos-eof (position 2 1))
-        (equal pstate1
-               (change-parstate
-                pstate0
-                :bytes (list 10 66)
-                :position (position 1 1)
-                :chars-read (list (char+position 65 (position 1 0)))
-                :size 2))
-        (equal pstate2
-               (change-parstate
-                pstate1
-                :bytes (list 66)
-                :position (position 2 0)
-                :chars-read (list (char+position 10 (position 1 1))
-                                  (char+position 65 (position 1 0)))
-                :size 1))
-        (equal pstate3
-               (change-parstate
-                pstate2
-                :chars-read nil
-                :chars-unread (list (char+position 65 (position 1 0))
-                                    (char+position 10 (position 1 1)))
-                :size 3))
-        (equal pstate4
-               (change-parstate
-                pstate3
-                :chars-read (list (char+position 65 (position 1 0)))
-                :chars-unread (list (char+position 10 (position 1 1)))
-                :size 2))
-        (equal pstate5
-               (change-parstate
-                pstate4
-                :chars-read (list (char+position 10 (position 1 1))
-                                  (char+position 65 (position 1 0)))
-                :chars-unread nil
-                :size 1))
-        (equal pstate6
-               (change-parstate
-                pstate5
-                :chars-read (list (char+position 65 (position 1 0)))
-                :chars-unread (list (char+position 10 (position 1 1)))
-                :size 2))
-        (equal pstate7
-               (change-parstate
-                pstate6
-                :chars-read (list (char+position 10 (position 1 1))
-                                  (char+position 65 (position 1 0)))
-                :chars-unread nil
-                :size 1))
-        (equal pstate8
-               (change-parstate
-                pstate7
-                :bytes nil
-                :position (position 2 1)
-                :chars-read (list (char+position 66 (position 2 0))
-                                  (char+position 10 (position 1 1))
-                                  (char+position 65 (position 1 0)))
-                :size 0))
-        (equal pstate9
-               pstate8))))
+(assert!-stobj
+ (b* ((parstate (init-parstate (list 65 10 66) nil parstate)) ; A LF B
+      (pstate0 (to-parstate$ parstate))
+      ((mv erp1 char-a pos-a parstate) (read-char parstate))
+      (pstate1 (to-parstate$ parstate))
+      ((mv erp2 char-nl pos-nl parstate) (read-char parstate))
+      (pstate2 (to-parstate$ parstate))
+      (parstate (unread-chars 2 parstate))
+      (pstate3 (to-parstate$ parstate))
+      ((mv erp4 char-a2 pos-a2 parstate) (read-char parstate))
+      (pstate4 (to-parstate$ parstate))
+      ((mv erp5 char-nl2 pos-nl2 parstate) (read-char parstate))
+      (pstate5 (to-parstate$ parstate))
+      (parstate (unread-char parstate))
+      (pstate6 (to-parstate$ parstate))
+      ((mv erp7 char-nl3 pos-nl3 parstate) (read-char parstate))
+      (pstate7 (to-parstate$ parstate))
+      ((mv erp8 char-b pos-b parstate) (read-char parstate))
+      (pstate8 (to-parstate$ parstate))
+      ((mv erp9 char-eof pos-eof parstate) (read-char parstate))
+      (pstate9 (to-parstate$ parstate)))
+   (mv (and (not erp1)
+            (not erp2)
+            (not erp4)
+            (not erp5)
+            (not erp7)
+            (not erp8)
+            (not erp9)
+            (equal char-a 65)
+            (equal char-nl 10)
+            (equal char-a2 65)
+            (equal char-nl2 10)
+            (equal char-nl3 10)
+            (equal char-b 66)
+            (equal char-eof nil)
+            (equal pos-a (position 1 0))
+            (equal pos-a2 (position 1 0))
+            (equal pos-nl (position 1 1))
+            (equal pos-nl2 (position 1 1))
+            (equal pos-nl3 (position 1 1))
+            (equal pos-b (position 2 0))
+            (equal pos-eof (position 2 1))
+            (equal pstate1
+                   (change-parstate$
+                    pstate0
+                    :bytes (list 10 66)
+                    :position (position 1 1)
+                    :chars-read (list (char+position 65 (position 1 0)))
+                    :size 2))
+            (equal pstate2
+                   (change-parstate$
+                    pstate1
+                    :bytes (list 66)
+                    :position (position 2 0)
+                    :chars-read (list (char+position 10 (position 1 1))
+                                      (char+position 65 (position 1 0)))
+                    :size 1))
+            (equal pstate3
+                   (change-parstate$
+                    pstate2
+                    :chars-read nil
+                    :chars-unread (list (char+position 65 (position 1 0))
+                                        (char+position 10 (position 1 1)))
+                    :size 3))
+            (equal pstate4
+                   (change-parstate$
+                    pstate3
+                    :chars-read (list (char+position 65 (position 1 0)))
+                    :chars-unread (list (char+position 10 (position 1 1)))
+                    :size 2))
+            (equal pstate5
+                   (change-parstate$
+                    pstate4
+                    :chars-read (list (char+position 10 (position 1 1))
+                                      (char+position 65 (position 1 0)))
+                    :chars-unread nil
+                    :size 1))
+            (equal pstate6
+                   (change-parstate$
+                    pstate5
+                    :chars-read (list (char+position 65 (position 1 0)))
+                    :chars-unread (list (char+position 10 (position 1 1)))
+                    :size 2))
+            (equal pstate7
+                   (change-parstate$
+                    pstate6
+                    :chars-read (list (char+position 10 (position 1 1))
+                                      (char+position 65 (position 1 0)))
+                    :chars-unread nil
+                    :size 1))
+            (equal pstate8
+                   (change-parstate$
+                    pstate7
+                    :bytes nil
+                    :position (position 2 1)
+                    :chars-read (list (char+position 66 (position 2 0))
+                                      (char+position 10 (position 1 1))
+                                      (char+position 65 (position 1 0)))
+                    :size 0))
+            (equal pstate9
+                   pstate8))
+       parstate))
+ parstate)
 
 ;;;;;;;;;;;;;;;;;;;;;;;;;;;;;;;;;;;;;;;;;;;;;;;;;;;;;;;;;;;;;;;;;;;;;;;;;;;;;;;;
 
@@ -521,42 +597,48 @@
   ;; where the term evaluates to a string or a list of bytes.
   ;; Optional POS is the initial position for the parser state.
   ;; Optional MORE-INPUTS go just before parser state input.
-  ;; Optional COND may be over variables AST, POS/SPAN, PSTATE,
-  ;; and also POS/SPAN2 for LEX-*-DIGIT.
-  `(assert-event
-    (b* ((pstate (init-parstate (if (stringp ,input)
-                                    (acl2::string=>nats ,input)
-                                  ,input)
-                                nil))
+  ;; Optional COND may be over variables AST, POS/SPAN, PARSTATE,
+  ;; and also POS/SPAN2 for LEX-*-DIGIT and LEX-*-HEXADECIMAL-DIGIT.
+  `(assert!-stobj
+    (b* ((parstate (init-parstate (if (stringp ,input)
+                                      (acl2::string=>nats ,input)
+                                    ,input)
+                                  nil
+                                  parstate))
          ,@(and pos
-                `((pstate (change-parstate pstate :position ,pos))))
+                `((parstate (update-parstate->position ,pos parstate))))
          (,(if (member-eq fn '(lex-*-digit
                                lex-*-hexadecimal-digit))
-               '(mv erp ?ast ?pos/span ?pos/span2 ?pstate)
-             '(mv erp ?ast ?pos/span ?pstate))
-          (,fn ,@more-inputs pstate)))
-      (if erp
-          (cw "~@0" erp) ; CW returns NIL, so ASSERT-EVENT fails
-        ,(or cond t))))) ; ASSERT-EVENT passes if COND is absent or else holds
+               '(mv erp ?ast ?pos/span ?pos/span2 parstate)
+             '(mv erp ?ast ?pos/span parstate))
+          (,fn ,@more-inputs parstate)))
+      (mv
+       (if erp
+           (cw "~@0" erp) ; CW returns NIL, so ASSERT!-STOBJ fails
+         ,(or cond t)) ; assertion passes if COND is absent or else holds
+       parstate))
+    parstate))
 
 (defmacro test-lex-fail (fn input &key pos more-inputs)
   ;; INPUT is an ACL2 term with the text to lex,
   ;; where the term evaluates to a string or a list of bytes.
   ;; Optional POS is the initial position for the parser state.
   ;; Optional MORE-INPUTS go just before parser state input.
-  `(assert-event
-    (b* ((pstate (init-parstate (if (stringp ,input)
-                                    (acl2::string=>nats ,input)
-                                  ,input)
-                                nil))
+  `(assert!-stobj
+    (b* ((parstate (init-parstate (if (stringp ,input)
+                                      (acl2::string=>nats ,input)
+                                    ,input)
+                                  nil
+                                  parstate))
          ,@(and pos
-                `((pstate (change-parstate pstate :position ,pos))))
+                `((parstate (update-parstate->position ,pos parstate))))
          (,(if (member-eq fn '(lex-*-digit
                                lex-*-hexadecimal-digit))
-               '(mv erp & & & &)
-             '(mv erp & & &))
-          (,fn ,@more-inputs pstate)))
-      erp)))
+               '(mv erp & & & parstate)
+             '(mv erp & & parstate))
+          (,fn ,@more-inputs parstate)))
+      (mv erp parstate))
+    parstate))
 
 ;;;;;;;;;;;;;;;;;;;;;;;;;;;;;;;;;;;;;;;;
 
@@ -611,7 +693,7 @@
  lex-hexadecimal-digit
  "fy"
  :cond (and (equal ast #\f)
-            (equal (parstate->bytes pstate) (list (char-code #\y)))))
+            (equal (parstate->bytes parstate) (list (char-code #\y)))))
 
 (test-lex-fail
  lex-hexadecimal-digit
@@ -651,7 +733,7 @@
  lex-hex-quad
  "DeadBeef"
  :cond (and (equal ast (hex-quad #\D #\e #\a #\d))
-            (equal (parstate->bytes pstate) (acl2::string=>nats "Beef"))))
+            (equal (parstate->bytes parstate) (acl2::string=>nats "Beef"))))
 
 (test-lex-fail
  lex-hex-quad
@@ -1030,16 +1112,19 @@
 (defmacro test-parse (fn input &key cond gcc)
   ;; Input is an ACL2 term with the text to parse,
   ;; where the term evaluates to a string or a list of bytes.
-  ;; Optional COND may be over variables AST, SPAN, PSTATE
+  ;; Optional COND may be over variables AST, SPAN, PARSTATE
   ;; and also EOF-POS for PARSE-EXTERNAL-DECLARATION-LIST.
-  `(assert-event
-    (b* ((,(if (eq fn 'parse-external-declaration-list)
-               '(mv erp ?ast ?span ?eofpos ?pstate)
-             '(mv erp ?ast ?span ?pstate))
-          (,fn (init-parstate (acl2::string=>nats ,input) ,gcc))))
-      (if erp
-          (cw "~@0" erp) ; CW returns NIL, so ASSERT-EVENT fails
-        ,(or cond t))))) ; ASSERT-EVENT passes if COND is absent or else holds
+  `(assert!-stobj
+    (b* ((parstate (init-parstate (acl2::string=>nats ,input) ,gcc parstate))
+         (,(if (eq fn 'parse-external-declaration-list)
+               '(mv erp ?ast ?span ?eofpos parstate)
+             '(mv erp ?ast ?span parstate))
+          (,fn parstate)))
+      (mv (if erp
+              (cw "~@0" erp) ; CW returns NIL, so ASSERT!-STOBJ fails
+            ,(or cond t)) ; assertion passes if COND is absent or else holds
+          parstate))
+    parstate))
 
 ;;;;;;;;;;;;;;;;;;;;;;;;;;;;;;;;;;;;;;;;
 
